Organize the code

dorami/code/Sally_Port.s
@@ -1,10 +1,10 @@
 sallyport_entry:
     csrci mstatus, 0x08
 
-    li t0, 0x8001FFD4
+    li t0, 0x80000000
     csrw mtvec, t0
 
     li t0, 0x9B989D989D1E
     csrw pmpcfg0, t0
 
-    jal zero, -0x10816
+    jal zero, -0x21034
