dorami/instructions/Sally_Port/a0.v
@@ -6,154 +6,172 @@ Definition a0 : isla_trace :=
   Assume (AExp_Binop (Eq) (AExp_Val (AVal_Var "cur_privilege" []) Mk_annot) (AExp_Val (AVal_Var "Machine" []) Mk_annot) Mk_annot) Mk_annot :t:
   Smt (DeclareConst 1%Z (Ty_BitVec 64%N)) Mk_annot :t:
   Assume (AExp_Binop (Eq) (AExp_Val (AVal_Var "misa" [Field "bits"]) Mk_annot) (AExp_Val (AVal_Bits (BV 64%N 0x800000000015312d%Z)) Mk_annot) Mk_annot) Mk_annot :t:
-  Smt (DeclareConst 2%Z (Ty_BitVec 64%N)) Mk_annot :t:
-  ReadReg "PC" [] (RegVal_Base (Val_Symbolic 2%Z)) Mk_annot :t:
-  Smt (DefineConst 3%Z (Manyop (Bvmanyarith Bvadd) [Val (Val_Symbolic 2%Z) Mk_annot; Val (Val_Bits (BV 64%N 0x4%Z)) Mk_annot] Mk_annot)) Mk_annot :t:
+  Smt (DeclareConst 2%Z (Ty_BitVec 8%N)) Mk_annot :t:
+  Assume (AExp_Binop (Eq) (AExp_Val (AVal_Var "pmp0cfg" [Field "bits"]) Mk_annot) (AExp_Val (AVal_Bits (BV 8%N 0x0%Z)) Mk_annot) Mk_annot) Mk_annot :t:
+  Smt (DeclareConst 3%Z (Ty_BitVec 8%N)) Mk_annot :t:
+  Assume (AExp_Binop (Eq) (AExp_Val (AVal_Var "pmp1cfg" [Field "bits"]) Mk_annot) (AExp_Val (AVal_Bits (BV 8%N 0x0%Z)) Mk_annot) Mk_annot) Mk_annot :t:
+  Smt (DeclareConst 4%Z (Ty_BitVec 8%N)) Mk_annot :t:
+  Assume (AExp_Binop (Eq) (AExp_Val (AVal_Var "pmp2cfg" [Field "bits"]) Mk_annot) (AExp_Val (AVal_Bits (BV 8%N 0x0%Z)) Mk_annot) Mk_annot) Mk_annot :t:
+  Smt (DeclareConst 5%Z (Ty_BitVec 8%N)) Mk_annot :t:
+  Assume (AExp_Binop (Eq) (AExp_Val (AVal_Var "pmp3cfg" [Field "bits"]) Mk_annot) (AExp_Val (AVal_Bits (BV 8%N 0x0%Z)) Mk_annot) Mk_annot) Mk_annot :t:
+  Smt (DeclareConst 6%Z (Ty_BitVec 8%N)) Mk_annot :t:
+  Assume (AExp_Binop (Eq) (AExp_Val (AVal_Var "pmp4cfg" [Field "bits"]) Mk_annot) (AExp_Val (AVal_Bits (BV 8%N 0x0%Z)) Mk_annot) Mk_annot) Mk_annot :t:
+  Smt (DeclareConst 7%Z (Ty_BitVec 8%N)) Mk_annot :t:
+  Assume (AExp_Binop (Eq) (AExp_Val (AVal_Var "pmp5cfg" [Field "bits"]) Mk_annot) (AExp_Val (AVal_Bits (BV 8%N 0x0%Z)) Mk_annot) Mk_annot) Mk_annot :t:
+  Smt (DeclareConst 8%Z (Ty_BitVec 8%N)) Mk_annot :t:
+  Assume (AExp_Binop (Eq) (AExp_Val (AVal_Var "pmp6cfg" [Field "bits"]) Mk_annot) (AExp_Val (AVal_Bits (BV 8%N 0x0%Z)) Mk_annot) Mk_annot) Mk_annot :t:
+  Smt (DeclareConst 9%Z (Ty_BitVec 8%N)) Mk_annot :t:
+  Assume (AExp_Binop (Eq) (AExp_Val (AVal_Var "pmp7cfg" [Field "bits"]) Mk_annot) (AExp_Val (AVal_Bits (BV 8%N 0x0%Z)) Mk_annot) Mk_annot) Mk_annot :t:
+  Smt (DeclareConst 10%Z (Ty_BitVec 64%N)) Mk_annot :t:
+  Assume (AExp_Binop (Eq) (AExp_Val (AVal_Var "mseccfg" [Field "bits"]) Mk_annot) (AExp_Val (AVal_Bits (BV 64%N 0x7%Z)) Mk_annot) Mk_annot) Mk_annot :t:
+  Smt (DeclareConst 11%Z (Ty_BitVec 64%N)) Mk_annot :t:
+  ReadReg "PC" [] (RegVal_Base (Val_Symbolic 11%Z)) Mk_annot :t:
+  Smt (DefineConst 12%Z (Manyop (Bvmanyarith Bvadd) [Val (Val_Symbolic 11%Z) Mk_annot; Val (Val_Bits (BV 64%N 0x4%Z)) Mk_annot] Mk_annot)) Mk_annot :t:
   ReadReg "cur_privilege" [] (RegVal_Base (Val_Symbolic 0%Z)) Mk_annot :t:
-  Smt (DeclareConst 14%Z (Ty_BitVec 64%N)) Mk_annot :t:
-  ReadReg "mstatus" [Field "bits"] (RegVal_Struct [("bits", RegVal_Base (Val_Symbolic 14%Z))]) Mk_annot :t:
-  Smt (DefineConst 15%Z (Manyop (Bvmanyarith Bvand) [Val (Val_Symbolic 14%Z) Mk_annot; Val (Val_Bits (BV 64%N 0xfffffffffffffff7%Z)) Mk_annot] Mk_annot)) Mk_annot :t:
-  ReadReg "mstatus" [Field "bits"] (RegVal_Struct [("bits", RegVal_Base (Val_Symbolic 14%Z))]) Mk_annot :t:
-  Smt (DefineConst 24%Z (Manyop (Bvmanyarith Bvand) [Unop (ZeroExtend 41%N) (Manyop Concat [Unop (Extract 22%N 7%N) (Val (Val_Symbolic 15%Z) Mk_annot) Mk_annot; Manyop Concat [Val (Val_Bits (BV 1%N 0x0%Z)) Mk_annot; Manyop Concat [Unop (Extract 5%N 3%N) (Val (Val_Symbolic 15%Z) Mk_annot) Mk_annot; Manyop Concat [Val (Val_Bits (BV 1%N 0x0%Z)) Mk_annot; Unop (Extract 1%N 0%N) (Val (Val_Symbolic 15%Z) Mk_annot) Mk_annot] Mk_annot] Mk_annot] Mk_annot] Mk_annot) Mk_annot; Val (Val_Bits (BV 64%N 0xfffffffffffe7fff%Z)) Mk_annot] Mk_annot)) Mk_annot :t:
-  Smt (DefineConst 25%Z (Unop (Extract 14%N 13%N) (Val (Val_Symbolic 24%Z) Mk_annot) Mk_annot)) Mk_annot :t:
-  Smt (DefineConst 27%Z (Unop (Not) (Binop (Eq) (Val (Val_Symbolic 25%Z) Mk_annot) (Val (Val_Bits (BV 2%N 0x0%Z)) Mk_annot) Mk_annot) Mk_annot)) Mk_annot :t:
+  Smt (DeclareConst 23%Z (Ty_BitVec 64%N)) Mk_annot :t:
+  ReadReg "mstatus" [Field "bits"] (RegVal_Struct [("bits", RegVal_Base (Val_Symbolic 23%Z))]) Mk_annot :t:
+  Smt (DefineConst 24%Z (Manyop (Bvmanyarith Bvand) [Val (Val_Symbolic 23%Z) Mk_annot; Val (Val_Bits (BV 64%N 0xfffffffffffffff7%Z)) Mk_annot] Mk_annot)) Mk_annot :t:
+  ReadReg "mstatus" [Field "bits"] (RegVal_Struct [("bits", RegVal_Base (Val_Symbolic 23%Z))]) Mk_annot :t:
+  Smt (DefineConst 33%Z (Manyop (Bvmanyarith Bvand) [Unop (ZeroExtend 41%N) (Manyop Concat [Unop (Extract 22%N 7%N) (Val (Val_Symbolic 24%Z) Mk_annot) Mk_annot; Manyop Concat [Val (Val_Bits (BV 1%N 0x0%Z)) Mk_annot; Manyop Concat [Unop (Extract 5%N 3%N) (Val (Val_Symbolic 24%Z) Mk_annot) Mk_annot; Manyop Concat [Val (Val_Bits (BV 1%N 0x0%Z)) Mk_annot; Unop (Extract 1%N 0%N) (Val (Val_Symbolic 24%Z) Mk_annot) Mk_annot] Mk_annot] Mk_annot] Mk_annot] Mk_annot) Mk_annot; Val (Val_Bits (BV 64%N 0xfffffffffffe7fff%Z)) Mk_annot] Mk_annot)) Mk_annot :t:
+  Smt (DefineConst 34%Z (Unop (Extract 14%N 13%N) (Val (Val_Symbolic 33%Z) Mk_annot) Mk_annot)) Mk_annot :t:
+  Smt (DefineConst 36%Z (Unop (Not) (Binop (Eq) (Val (Val_Symbolic 34%Z) Mk_annot) (Val (Val_Bits (BV 2%N 0x0%Z)) Mk_annot) Mk_annot) Mk_annot)) Mk_annot :t:
   tcases [
-    Smt (Assert (Val (Val_Symbolic 27%Z) Mk_annot)) Mk_annot :t:
-    Smt (DefineConst 29%Z (Unop (Not) (Binop (Eq) (Val (Val_Symbolic 25%Z) Mk_annot) (Val (Val_Bits (BV 2%N 0x1%Z)) Mk_annot) Mk_annot) Mk_annot)) Mk_annot :t:
+    Smt (Assert (Val (Val_Symbolic 36%Z) Mk_annot)) Mk_annot :t:
+    Smt (DefineConst 38%Z (Unop (Not) (Binop (Eq) (Val (Val_Symbolic 34%Z) Mk_annot) (Val (Val_Bits (BV 2%N 0x1%Z)) Mk_annot) Mk_annot) Mk_annot)) Mk_annot :t:
     tcases [
-      Smt (Assert (Val (Val_Symbolic 29%Z) Mk_annot)) Mk_annot :t:
-      Smt (DefineConst 31%Z (Unop (Not) (Binop (Eq) (Val (Val_Symbolic 25%Z) Mk_annot) (Val (Val_Bits (BV 2%N 0x2%Z)) Mk_annot) Mk_annot) Mk_annot)) Mk_annot :t:
+      Smt (Assert (Val (Val_Symbolic 38%Z) Mk_annot)) Mk_annot :t:
+      Smt (DefineConst 40%Z (Unop (Not) (Binop (Eq) (Val (Val_Symbolic 34%Z) Mk_annot) (Val (Val_Bits (BV 2%N 0x2%Z)) Mk_annot) Mk_annot) Mk_annot)) Mk_annot :t:
       tcases [
-        Smt (Assert (Val (Val_Symbolic 31%Z) Mk_annot)) Mk_annot :t:
-        Smt (DefineConst 37%Z (Manyop (Bvmanyarith Bvand) [Manyop (Bvmanyarith Bvor) [Manyop (Bvmanyarith Bvand) [Manyop (Bvmanyarith Bvor) [Manyop (Bvmanyarith Bvand) [Manyop (Bvmanyarith Bvor) [Manyop (Bvmanyarith Bvand) [Val (Val_Symbolic 24%Z) Mk_annot; Val (Val_Bits (BV 64%N 0x7fffffffffffffff%Z)) Mk_annot] Mk_annot; Val (Val_Bits (BV 64%N 0x8000000000000000%Z)) Mk_annot] Mk_annot; Val (Val_Bits (BV 64%N 0xfffffff3ffffffff%Z)) Mk_annot] Mk_annot; Binop ((Bvarith Bvshl)) (Unop (ZeroExtend 62%N) (Unop (Extract 35%N 34%N) (Val (Val_Symbolic 14%Z) Mk_annot) Mk_annot) Mk_annot) (Val (Val_Bits (BV 64%N 0x22%Z)) Mk_annot) Mk_annot] Mk_annot; Val (Val_Bits (BV 64%N 0xfffffffcffffffff%Z)) Mk_annot] Mk_annot; Binop ((Bvarith Bvshl)) (Unop (ZeroExtend 62%N) (Unop (Extract 33%N 32%N) (Val (Val_Symbolic 14%Z) Mk_annot) Mk_annot) Mk_annot) (Val (Val_Bits (BV 64%N 0x20%Z)) Mk_annot) Mk_annot] Mk_annot; Val (Val_Bits (BV 64%N 0xffffffcfffffffff%Z)) Mk_annot] Mk_annot)) Mk_annot :t:
+        Smt (Assert (Val (Val_Symbolic 40%Z) Mk_annot)) Mk_annot :t:
+        Smt (DefineConst 46%Z (Manyop (Bvmanyarith Bvand) [Manyop (Bvmanyarith Bvor) [Manyop (Bvmanyarith Bvand) [Manyop (Bvmanyarith Bvor) [Manyop (Bvmanyarith Bvand) [Manyop (Bvmanyarith Bvor) [Manyop (Bvmanyarith Bvand) [Val (Val_Symbolic 33%Z) Mk_annot; Val (Val_Bits (BV 64%N 0x7fffffffffffffff%Z)) Mk_annot] Mk_annot; Val (Val_Bits (BV 64%N 0x8000000000000000%Z)) Mk_annot] Mk_annot; Val (Val_Bits (BV 64%N 0xfffffff3ffffffff%Z)) Mk_annot] Mk_annot; Binop ((Bvarith Bvshl)) (Unop (ZeroExtend 62%N) (Unop (Extract 35%N 34%N) (Val (Val_Symbolic 23%Z) Mk_annot) Mk_annot) Mk_annot) (Val (Val_Bits (BV 64%N 0x22%Z)) Mk_annot) Mk_annot] Mk_annot; Val (Val_Bits (BV 64%N 0xfffffffcffffffff%Z)) Mk_annot] Mk_annot; Binop ((Bvarith Bvshl)) (Unop (ZeroExtend 62%N) (Unop (Extract 33%N 32%N) (Val (Val_Symbolic 23%Z) Mk_annot) Mk_annot) Mk_annot) (Val (Val_Bits (BV 64%N 0x20%Z)) Mk_annot) Mk_annot] Mk_annot; Val (Val_Bits (BV 64%N 0xffffffcfffffffff%Z)) Mk_annot] Mk_annot)) Mk_annot :t:
         ReadReg "misa" [Field "bits"] (RegVal_Struct [("bits", RegVal_Base (Val_Symbolic 1%Z))]) Mk_annot :t:
-        WriteReg "mstatus" [Field "bits"] (RegVal_Struct [("bits", RegVal_Base (Val_Symbolic 37%Z))]) Mk_annot :t:
-        ReadReg "mstatus" [Field "bits"] (RegVal_Struct [("bits", RegVal_Base (Val_Symbolic 37%Z))]) Mk_annot :t:
-        WriteReg "PC" [] (RegVal_Base (Val_Symbolic 3%Z)) Mk_annot :t:
+        WriteReg "mstatus" [Field "bits"] (RegVal_Struct [("bits", RegVal_Base (Val_Symbolic 46%Z))]) Mk_annot :t:
+        ReadReg "mstatus" [Field "bits"] (RegVal_Struct [("bits", RegVal_Base (Val_Symbolic 46%Z))]) Mk_annot :t:
+        WriteReg "PC" [] (RegVal_Base (Val_Symbolic 12%Z)) Mk_annot :t:
         tnil;
-        Smt (Assert (Unop (Not) (Val (Val_Symbolic 31%Z) Mk_annot) Mk_annot)) Mk_annot :t:
-        Smt (DefineConst 47%Z (Unop (Extract 10%N 9%N) (Val (Val_Symbolic 24%Z) Mk_annot) Mk_annot)) Mk_annot :t:
-        Smt (DefineConst 49%Z (Unop (Not) (Binop (Eq) (Val (Val_Symbolic 47%Z) Mk_annot) (Val (Val_Bits (BV 2%N 0x0%Z)) Mk_annot) Mk_annot) Mk_annot)) Mk_annot :t:
+        Smt (Assert (Unop (Not) (Val (Val_Symbolic 40%Z) Mk_annot) Mk_annot)) Mk_annot :t:
+        Smt (DefineConst 56%Z (Unop (Extract 10%N 9%N) (Val (Val_Symbolic 33%Z) Mk_annot) Mk_annot)) Mk_annot :t:
+        Smt (DefineConst 58%Z (Unop (Not) (Binop (Eq) (Val (Val_Symbolic 56%Z) Mk_annot) (Val (Val_Bits (BV 2%N 0x0%Z)) Mk_annot) Mk_annot) Mk_annot)) Mk_annot :t:
         tcases [
-          Smt (Assert (Val (Val_Symbolic 49%Z) Mk_annot)) Mk_annot :t:
-          Smt (DefineConst 51%Z (Unop (Not) (Binop (Eq) (Val (Val_Symbolic 47%Z) Mk_annot) (Val (Val_Bits (BV 2%N 0x1%Z)) Mk_annot) Mk_annot) Mk_annot)) Mk_annot :t:
+          Smt (Assert (Val (Val_Symbolic 58%Z) Mk_annot)) Mk_annot :t:
+          Smt (DefineConst 60%Z (Unop (Not) (Binop (Eq) (Val (Val_Symbolic 56%Z) Mk_annot) (Val (Val_Bits (BV 2%N 0x1%Z)) Mk_annot) Mk_annot) Mk_annot)) Mk_annot :t:
           tcases [
-            Smt (Assert (Val (Val_Symbolic 51%Z) Mk_annot)) Mk_annot :t:
-            Smt (DefineConst 53%Z (Unop (Not) (Binop (Eq) (Val (Val_Symbolic 47%Z) Mk_annot) (Val (Val_Bits (BV 2%N 0x2%Z)) Mk_annot) Mk_annot) Mk_annot)) Mk_annot :t:
+            Smt (Assert (Val (Val_Symbolic 60%Z) Mk_annot)) Mk_annot :t:
+            Smt (DefineConst 62%Z (Unop (Not) (Binop (Eq) (Val (Val_Symbolic 56%Z) Mk_annot) (Val (Val_Bits (BV 2%N 0x2%Z)) Mk_annot) Mk_annot) Mk_annot)) Mk_annot :t:
             tcases [
-              Smt (Assert (Val (Val_Symbolic 53%Z) Mk_annot)) Mk_annot :t:
-              Smt (DefineConst 59%Z (Manyop (Bvmanyarith Bvand) [Manyop (Bvmanyarith Bvor) [Manyop (Bvmanyarith Bvand) [Manyop (Bvmanyarith Bvor) [Manyop (Bvmanyarith Bvand) [Manyop (Bvmanyarith Bvor) [Manyop (Bvmanyarith Bvand) [Val (Val_Symbolic 24%Z) Mk_annot; Val (Val_Bits (BV 64%N 0x7fffffffffffffff%Z)) Mk_annot] Mk_annot; Val (Val_Bits (BV 64%N 0x8000000000000000%Z)) Mk_annot] Mk_annot; Val (Val_Bits (BV 64%N 0xfffffff3ffffffff%Z)) Mk_annot] Mk_annot; Binop ((Bvarith Bvshl)) (Unop (ZeroExtend 62%N) (Unop (Extract 35%N 34%N) (Val (Val_Symbolic 14%Z) Mk_annot) Mk_annot) Mk_annot) (Val (Val_Bits (BV 64%N 0x22%Z)) Mk_annot) Mk_annot] Mk_annot; Val (Val_Bits (BV 64%N 0xfffffffcffffffff%Z)) Mk_annot] Mk_annot; Binop ((Bvarith Bvshl)) (Unop (ZeroExtend 62%N) (Unop (Extract 33%N 32%N) (Val (Val_Symbolic 14%Z) Mk_annot) Mk_annot) Mk_annot) (Val (Val_Bits (BV 64%N 0x20%Z)) Mk_annot) Mk_annot] Mk_annot; Val (Val_Bits (BV 64%N 0xffffffcfffffffff%Z)) Mk_annot] Mk_annot)) Mk_annot :t:
+              Smt (Assert (Val (Val_Symbolic 62%Z) Mk_annot)) Mk_annot :t:
+              Smt (DefineConst 68%Z (Manyop (Bvmanyarith Bvand) [Manyop (Bvmanyarith Bvor) [Manyop (Bvmanyarith Bvand) [Manyop (Bvmanyarith Bvor) [Manyop (Bvmanyarith Bvand) [Manyop (Bvmanyarith Bvor) [Manyop (Bvmanyarith Bvand) [Val (Val_Symbolic 33%Z) Mk_annot; Val (Val_Bits (BV 64%N 0x7fffffffffffffff%Z)) Mk_annot] Mk_annot; Val (Val_Bits (BV 64%N 0x8000000000000000%Z)) Mk_annot] Mk_annot; Val (Val_Bits (BV 64%N 0xfffffff3ffffffff%Z)) Mk_annot] Mk_annot; Binop ((Bvarith Bvshl)) (Unop (ZeroExtend 62%N) (Unop (Extract 35%N 34%N) (Val (Val_Symbolic 23%Z) Mk_annot) Mk_annot) Mk_annot) (Val (Val_Bits (BV 64%N 0x22%Z)) Mk_annot) Mk_annot] Mk_annot; Val (Val_Bits (BV 64%N 0xfffffffcffffffff%Z)) Mk_annot] Mk_annot; Binop ((Bvarith Bvshl)) (Unop (ZeroExtend 62%N) (Unop (Extract 33%N 32%N) (Val (Val_Symbolic 23%Z) Mk_annot) Mk_annot) Mk_annot) (Val (Val_Bits (BV 64%N 0x20%Z)) Mk_annot) Mk_annot] Mk_annot; Val (Val_Bits (BV 64%N 0xffffffcfffffffff%Z)) Mk_annot] Mk_annot)) Mk_annot :t:
               ReadReg "misa" [Field "bits"] (RegVal_Struct [("bits", RegVal_Base (Val_Symbolic 1%Z))]) Mk_annot :t:
-              WriteReg "mstatus" [Field "bits"] (RegVal_Struct [("bits", RegVal_Base (Val_Symbolic 59%Z))]) Mk_annot :t:
-              ReadReg "mstatus" [Field "bits"] (RegVal_Struct [("bits", RegVal_Base (Val_Symbolic 59%Z))]) Mk_annot :t:
-              WriteReg "PC" [] (RegVal_Base (Val_Symbolic 3%Z)) Mk_annot :t:
+              WriteReg "mstatus" [Field "bits"] (RegVal_Struct [("bits", RegVal_Base (Val_Symbolic 68%Z))]) Mk_annot :t:
+              ReadReg "mstatus" [Field "bits"] (RegVal_Struct [("bits", RegVal_Base (Val_Symbolic 68%Z))]) Mk_annot :t:
+              WriteReg "PC" [] (RegVal_Base (Val_Symbolic 12%Z)) Mk_annot :t:
               tnil;
-              Smt (Assert (Unop (Not) (Val (Val_Symbolic 53%Z) Mk_annot) Mk_annot)) Mk_annot :t:
-              Smt (DefineConst 71%Z (Manyop (Bvmanyarith Bvand) [Manyop (Bvmanyarith Bvor) [Manyop (Bvmanyarith Bvand) [Manyop (Bvmanyarith Bvor) [Manyop (Bvmanyarith Bvand) [Manyop (Bvmanyarith Bvand) [Val (Val_Symbolic 24%Z) Mk_annot; Val (Val_Bits (BV 64%N 0x7fffffffffffffff%Z)) Mk_annot] Mk_annot; Val (Val_Bits (BV 64%N 0xfffffff3ffffffff%Z)) Mk_annot] Mk_annot; Binop ((Bvarith Bvshl)) (Unop (ZeroExtend 62%N) (Unop (Extract 35%N 34%N) (Val (Val_Symbolic 14%Z) Mk_annot) Mk_annot) Mk_annot) (Val (Val_Bits (BV 64%N 0x22%Z)) Mk_annot) Mk_annot] Mk_annot; Val (Val_Bits (BV 64%N 0xfffffffcffffffff%Z)) Mk_annot] Mk_annot; Binop ((Bvarith Bvshl)) (Unop (ZeroExtend 62%N) (Unop (Extract 33%N 32%N) (Val (Val_Symbolic 14%Z) Mk_annot) Mk_annot) Mk_annot) (Val (Val_Bits (BV 64%N 0x20%Z)) Mk_annot) Mk_annot] Mk_annot; Val (Val_Bits (BV 64%N 0xffffffcfffffffff%Z)) Mk_annot] Mk_annot)) Mk_annot :t:
+              Smt (Assert (Unop (Not) (Val (Val_Symbolic 62%Z) Mk_annot) Mk_annot)) Mk_annot :t:
+              Smt (DefineConst 80%Z (Manyop (Bvmanyarith Bvand) [Manyop (Bvmanyarith Bvor) [Manyop (Bvmanyarith Bvand) [Manyop (Bvmanyarith Bvor) [Manyop (Bvmanyarith Bvand) [Manyop (Bvmanyarith Bvand) [Val (Val_Symbolic 33%Z) Mk_annot; Val (Val_Bits (BV 64%N 0x7fffffffffffffff%Z)) Mk_annot] Mk_annot; Val (Val_Bits (BV 64%N 0xfffffff3ffffffff%Z)) Mk_annot] Mk_annot; Binop ((Bvarith Bvshl)) (Unop (ZeroExtend 62%N) (Unop (Extract 35%N 34%N) (Val (Val_Symbolic 23%Z) Mk_annot) Mk_annot) Mk_annot) (Val (Val_Bits (BV 64%N 0x22%Z)) Mk_annot) Mk_annot] Mk_annot; Val (Val_Bits (BV 64%N 0xfffffffcffffffff%Z)) Mk_annot] Mk_annot; Binop ((Bvarith Bvshl)) (Unop (ZeroExtend 62%N) (Unop (Extract 33%N 32%N) (Val (Val_Symbolic 23%Z) Mk_annot) Mk_annot) Mk_annot) (Val (Val_Bits (BV 64%N 0x20%Z)) Mk_annot) Mk_annot] Mk_annot; Val (Val_Bits (BV 64%N 0xffffffcfffffffff%Z)) Mk_annot] Mk_annot)) Mk_annot :t:
               ReadReg "misa" [Field "bits"] (RegVal_Struct [("bits", RegVal_Base (Val_Symbolic 1%Z))]) Mk_annot :t:
-              WriteReg "mstatus" [Field "bits"] (RegVal_Struct [("bits", RegVal_Base (Val_Symbolic 71%Z))]) Mk_annot :t:
-              ReadReg "mstatus" [Field "bits"] (RegVal_Struct [("bits", RegVal_Base (Val_Symbolic 71%Z))]) Mk_annot :t:
-              WriteReg "PC" [] (RegVal_Base (Val_Symbolic 3%Z)) Mk_annot :t:
+              WriteReg "mstatus" [Field "bits"] (RegVal_Struct [("bits", RegVal_Base (Val_Symbolic 80%Z))]) Mk_annot :t:
+              ReadReg "mstatus" [Field "bits"] (RegVal_Struct [("bits", RegVal_Base (Val_Symbolic 80%Z))]) Mk_annot :t:
+              WriteReg "PC" [] (RegVal_Base (Val_Symbolic 12%Z)) Mk_annot :t:
               tnil
             ];
-            Smt (Assert (Unop (Not) (Val (Val_Symbolic 51%Z) Mk_annot) Mk_annot)) Mk_annot :t:
-            Smt (DefineConst 83%Z (Manyop (Bvmanyarith Bvand) [Manyop (Bvmanyarith Bvor) [Manyop (Bvmanyarith Bvand) [Manyop (Bvmanyarith Bvor) [Manyop (Bvmanyarith Bvand) [Manyop (Bvmanyarith Bvand) [Val (Val_Symbolic 24%Z) Mk_annot; Val (Val_Bits (BV 64%N 0x7fffffffffffffff%Z)) Mk_annot] Mk_annot; Val (Val_Bits (BV 64%N 0xfffffff3ffffffff%Z)) Mk_annot] Mk_annot; Binop ((Bvarith Bvshl)) (Unop (ZeroExtend 62%N) (Unop (Extract 35%N 34%N) (Val (Val_Symbolic 14%Z) Mk_annot) Mk_annot) Mk_annot) (Val (Val_Bits (BV 64%N 0x22%Z)) Mk_annot) Mk_annot] Mk_annot; Val (Val_Bits (BV 64%N 0xfffffffcffffffff%Z)) Mk_annot] Mk_annot; Binop ((Bvarith Bvshl)) (Unop (ZeroExtend 62%N) (Unop (Extract 33%N 32%N) (Val (Val_Symbolic 14%Z) Mk_annot) Mk_annot) Mk_annot) (Val (Val_Bits (BV 64%N 0x20%Z)) Mk_annot) Mk_annot] Mk_annot; Val (Val_Bits (BV 64%N 0xffffffcfffffffff%Z)) Mk_annot] Mk_annot)) Mk_annot :t:
+            Smt (Assert (Unop (Not) (Val (Val_Symbolic 60%Z) Mk_annot) Mk_annot)) Mk_annot :t:
+            Smt (DefineConst 92%Z (Manyop (Bvmanyarith Bvand) [Manyop (Bvmanyarith Bvor) [Manyop (Bvmanyarith Bvand) [Manyop (Bvmanyarith Bvor) [Manyop (Bvmanyarith Bvand) [Manyop (Bvmanyarith Bvand) [Val (Val_Symbolic 33%Z) Mk_annot; Val (Val_Bits (BV 64%N 0x7fffffffffffffff%Z)) Mk_annot] Mk_annot; Val (Val_Bits (BV 64%N 0xfffffff3ffffffff%Z)) Mk_annot] Mk_annot; Binop ((Bvarith Bvshl)) (Unop (ZeroExtend 62%N) (Unop (Extract 35%N 34%N) (Val (Val_Symbolic 23%Z) Mk_annot) Mk_annot) Mk_annot) (Val (Val_Bits (BV 64%N 0x22%Z)) Mk_annot) Mk_annot] Mk_annot; Val (Val_Bits (BV 64%N 0xfffffffcffffffff%Z)) Mk_annot] Mk_annot; Binop ((Bvarith Bvshl)) (Unop (ZeroExtend 62%N) (Unop (Extract 33%N 32%N) (Val (Val_Symbolic 23%Z) Mk_annot) Mk_annot) Mk_annot) (Val (Val_Bits (BV 64%N 0x20%Z)) Mk_annot) Mk_annot] Mk_annot; Val (Val_Bits (BV 64%N 0xffffffcfffffffff%Z)) Mk_annot] Mk_annot)) Mk_annot :t:
             ReadReg "misa" [Field "bits"] (RegVal_Struct [("bits", RegVal_Base (Val_Symbolic 1%Z))]) Mk_annot :t:
-            WriteReg "mstatus" [Field "bits"] (RegVal_Struct [("bits", RegVal_Base (Val_Symbolic 83%Z))]) Mk_annot :t:
-            ReadReg "mstatus" [Field "bits"] (RegVal_Struct [("bits", RegVal_Base (Val_Symbolic 83%Z))]) Mk_annot :t:
-            WriteReg "PC" [] (RegVal_Base (Val_Symbolic 3%Z)) Mk_annot :t:
+            WriteReg "mstatus" [Field "bits"] (RegVal_Struct [("bits", RegVal_Base (Val_Symbolic 92%Z))]) Mk_annot :t:
+            ReadReg "mstatus" [Field "bits"] (RegVal_Struct [("bits", RegVal_Base (Val_Symbolic 92%Z))]) Mk_annot :t:
+            WriteReg "PC" [] (RegVal_Base (Val_Symbolic 12%Z)) Mk_annot :t:
             tnil
           ];
-          Smt (Assert (Unop (Not) (Val (Val_Symbolic 49%Z) Mk_annot) Mk_annot)) Mk_annot :t:
-          Smt (DefineConst 95%Z (Manyop (Bvmanyarith Bvand) [Manyop (Bvmanyarith Bvor) [Manyop (Bvmanyarith Bvand) [Manyop (Bvmanyarith Bvor) [Manyop (Bvmanyarith Bvand) [Manyop (Bvmanyarith Bvand) [Val (Val_Symbolic 24%Z) Mk_annot; Val (Val_Bits (BV 64%N 0x7fffffffffffffff%Z)) Mk_annot] Mk_annot; Val (Val_Bits (BV 64%N 0xfffffff3ffffffff%Z)) Mk_annot] Mk_annot; Binop ((Bvarith Bvshl)) (Unop (ZeroExtend 62%N) (Unop (Extract 35%N 34%N) (Val (Val_Symbolic 14%Z) Mk_annot) Mk_annot) Mk_annot) (Val (Val_Bits (BV 64%N 0x22%Z)) Mk_annot) Mk_annot] Mk_annot; Val (Val_Bits (BV 64%N 0xfffffffcffffffff%Z)) Mk_annot] Mk_annot; Binop ((Bvarith Bvshl)) (Unop (ZeroExtend 62%N) (Unop (Extract 33%N 32%N) (Val (Val_Symbolic 14%Z) Mk_annot) Mk_annot) Mk_annot) (Val (Val_Bits (BV 64%N 0x20%Z)) Mk_annot) Mk_annot] Mk_annot; Val (Val_Bits (BV 64%N 0xffffffcfffffffff%Z)) Mk_annot] Mk_annot)) Mk_annot :t:
+          Smt (Assert (Unop (Not) (Val (Val_Symbolic 58%Z) Mk_annot) Mk_annot)) Mk_annot :t:
+          Smt (DefineConst 104%Z (Manyop (Bvmanyarith Bvand) [Manyop (Bvmanyarith Bvor) [Manyop (Bvmanyarith Bvand) [Manyop (Bvmanyarith Bvor) [Manyop (Bvmanyarith Bvand) [Manyop (Bvmanyarith Bvand) [Val (Val_Symbolic 33%Z) Mk_annot; Val (Val_Bits (BV 64%N 0x7fffffffffffffff%Z)) Mk_annot] Mk_annot; Val (Val_Bits (BV 64%N 0xfffffff3ffffffff%Z)) Mk_annot] Mk_annot; Binop ((Bvarith Bvshl)) (Unop (ZeroExtend 62%N) (Unop (Extract 35%N 34%N) (Val (Val_Symbolic 23%Z) Mk_annot) Mk_annot) Mk_annot) (Val (Val_Bits (BV 64%N 0x22%Z)) Mk_annot) Mk_annot] Mk_annot; Val (Val_Bits (BV 64%N 0xfffffffcffffffff%Z)) Mk_annot] Mk_annot; Binop ((Bvarith Bvshl)) (Unop (ZeroExtend 62%N) (Unop (Extract 33%N 32%N) (Val (Val_Symbolic 23%Z) Mk_annot) Mk_annot) Mk_annot) (Val (Val_Bits (BV 64%N 0x20%Z)) Mk_annot) Mk_annot] Mk_annot; Val (Val_Bits (BV 64%N 0xffffffcfffffffff%Z)) Mk_annot] Mk_annot)) Mk_annot :t:
           ReadReg "misa" [Field "bits"] (RegVal_Struct [("bits", RegVal_Base (Val_Symbolic 1%Z))]) Mk_annot :t:
-          WriteReg "mstatus" [Field "bits"] (RegVal_Struct [("bits", RegVal_Base (Val_Symbolic 95%Z))]) Mk_annot :t:
-          ReadReg "mstatus" [Field "bits"] (RegVal_Struct [("bits", RegVal_Base (Val_Symbolic 95%Z))]) Mk_annot :t:
-          WriteReg "PC" [] (RegVal_Base (Val_Symbolic 3%Z)) Mk_annot :t:
+          WriteReg "mstatus" [Field "bits"] (RegVal_Struct [("bits", RegVal_Base (Val_Symbolic 104%Z))]) Mk_annot :t:
+          ReadReg "mstatus" [Field "bits"] (RegVal_Struct [("bits", RegVal_Base (Val_Symbolic 104%Z))]) Mk_annot :t:
+          WriteReg "PC" [] (RegVal_Base (Val_Symbolic 12%Z)) Mk_annot :t:
           tnil
         ]
       ];
-      Smt (Assert (Unop (Not) (Val (Val_Symbolic 29%Z) Mk_annot) Mk_annot)) Mk_annot :t:
-      Smt (DefineConst 105%Z (Unop (Extract 10%N 9%N) (Val (Val_Symbolic 24%Z) Mk_annot) Mk_annot)) Mk_annot :t:
-      Smt (DefineConst 107%Z (Unop (Not) (Binop (Eq) (Val (Val_Symbolic 105%Z) Mk_annot) (Val (Val_Bits (BV 2%N 0x0%Z)) Mk_annot) Mk_annot) Mk_annot)) Mk_annot :t:
+      Smt (Assert (Unop (Not) (Val (Val_Symbolic 38%Z) Mk_annot) Mk_annot)) Mk_annot :t:
+      Smt (DefineConst 114%Z (Unop (Extract 10%N 9%N) (Val (Val_Symbolic 33%Z) Mk_annot) Mk_annot)) Mk_annot :t:
+      Smt (DefineConst 116%Z (Unop (Not) (Binop (Eq) (Val (Val_Symbolic 114%Z) Mk_annot) (Val (Val_Bits (BV 2%N 0x0%Z)) Mk_annot) Mk_annot) Mk_annot)) Mk_annot :t:
       tcases [
-        Smt (Assert (Val (Val_Symbolic 107%Z) Mk_annot)) Mk_annot :t:
-        Smt (DefineConst 109%Z (Unop (Not) (Binop (Eq) (Val (Val_Symbolic 105%Z) Mk_annot) (Val (Val_Bits (BV 2%N 0x1%Z)) Mk_annot) Mk_annot) Mk_annot)) Mk_annot :t:
+        Smt (Assert (Val (Val_Symbolic 116%Z) Mk_annot)) Mk_annot :t:
+        Smt (DefineConst 118%Z (Unop (Not) (Binop (Eq) (Val (Val_Symbolic 114%Z) Mk_annot) (Val (Val_Bits (BV 2%N 0x1%Z)) Mk_annot) Mk_annot) Mk_annot)) Mk_annot :t:
         tcases [
-          Smt (Assert (Val (Val_Symbolic 109%Z) Mk_annot)) Mk_annot :t:
-          Smt (DefineConst 111%Z (Unop (Not) (Binop (Eq) (Val (Val_Symbolic 105%Z) Mk_annot) (Val (Val_Bits (BV 2%N 0x2%Z)) Mk_annot) Mk_annot) Mk_annot)) Mk_annot :t:
+          Smt (Assert (Val (Val_Symbolic 118%Z) Mk_annot)) Mk_annot :t:
+          Smt (DefineConst 120%Z (Unop (Not) (Binop (Eq) (Val (Val_Symbolic 114%Z) Mk_annot) (Val (Val_Bits (BV 2%N 0x2%Z)) Mk_annot) Mk_annot) Mk_annot)) Mk_annot :t:
           tcases [
-            Smt (Assert (Val (Val_Symbolic 111%Z) Mk_annot)) Mk_annot :t:
-            Smt (DefineConst 117%Z (Manyop (Bvmanyarith Bvand) [Manyop (Bvmanyarith Bvor) [Manyop (Bvmanyarith Bvand) [Manyop (Bvmanyarith Bvor) [Manyop (Bvmanyarith Bvand) [Manyop (Bvmanyarith Bvor) [Manyop (Bvmanyarith Bvand) [Val (Val_Symbolic 24%Z) Mk_annot; Val (Val_Bits (BV 64%N 0x7fffffffffffffff%Z)) Mk_annot] Mk_annot; Val (Val_Bits (BV 64%N 0x8000000000000000%Z)) Mk_annot] Mk_annot; Val (Val_Bits (BV 64%N 0xfffffff3ffffffff%Z)) Mk_annot] Mk_annot; Binop ((Bvarith Bvshl)) (Unop (ZeroExtend 62%N) (Unop (Extract 35%N 34%N) (Val (Val_Symbolic 14%Z) Mk_annot) Mk_annot) Mk_annot) (Val (Val_Bits (BV 64%N 0x22%Z)) Mk_annot) Mk_annot] Mk_annot; Val (Val_Bits (BV 64%N 0xfffffffcffffffff%Z)) Mk_annot] Mk_annot; Binop ((Bvarith Bvshl)) (Unop (ZeroExtend 62%N) (Unop (Extract 33%N 32%N) (Val (Val_Symbolic 14%Z) Mk_annot) Mk_annot) Mk_annot) (Val (Val_Bits (BV 64%N 0x20%Z)) Mk_annot) Mk_annot] Mk_annot; Val (Val_Bits (BV 64%N 0xffffffcfffffffff%Z)) Mk_annot] Mk_annot)) Mk_annot :t:
+            Smt (Assert (Val (Val_Symbolic 120%Z) Mk_annot)) Mk_annot :t:
+            Smt (DefineConst 126%Z (Manyop (Bvmanyarith Bvand) [Manyop (Bvmanyarith Bvor) [Manyop (Bvmanyarith Bvand) [Manyop (Bvmanyarith Bvor) [Manyop (Bvmanyarith Bvand) [Manyop (Bvmanyarith Bvor) [Manyop (Bvmanyarith Bvand) [Val (Val_Symbolic 33%Z) Mk_annot; Val (Val_Bits (BV 64%N 0x7fffffffffffffff%Z)) Mk_annot] Mk_annot; Val (Val_Bits (BV 64%N 0x8000000000000000%Z)) Mk_annot] Mk_annot; Val (Val_Bits (BV 64%N 0xfffffff3ffffffff%Z)) Mk_annot] Mk_annot; Binop ((Bvarith Bvshl)) (Unop (ZeroExtend 62%N) (Unop (Extract 35%N 34%N) (Val (Val_Symbolic 23%Z) Mk_annot) Mk_annot) Mk_annot) (Val (Val_Bits (BV 64%N 0x22%Z)) Mk_annot) Mk_annot] Mk_annot; Val (Val_Bits (BV 64%N 0xfffffffcffffffff%Z)) Mk_annot] Mk_annot; Binop ((Bvarith Bvshl)) (Unop (ZeroExtend 62%N) (Unop (Extract 33%N 32%N) (Val (Val_Symbolic 23%Z) Mk_annot) Mk_annot) Mk_annot) (Val (Val_Bits (BV 64%N 0x20%Z)) Mk_annot) Mk_annot] Mk_annot; Val (Val_Bits (BV 64%N 0xffffffcfffffffff%Z)) Mk_annot] Mk_annot)) Mk_annot :t:
             ReadReg "misa" [Field "bits"] (RegVal_Struct [("bits", RegVal_Base (Val_Symbolic 1%Z))]) Mk_annot :t:
-            WriteReg "mstatus" [Field "bits"] (RegVal_Struct [("bits", RegVal_Base (Val_Symbolic 117%Z))]) Mk_annot :t:
-            ReadReg "mstatus" [Field "bits"] (RegVal_Struct [("bits", RegVal_Base (Val_Symbolic 117%Z))]) Mk_annot :t:
-            WriteReg "PC" [] (RegVal_Base (Val_Symbolic 3%Z)) Mk_annot :t:
+            WriteReg "mstatus" [Field "bits"] (RegVal_Struct [("bits", RegVal_Base (Val_Symbolic 126%Z))]) Mk_annot :t:
+            ReadReg "mstatus" [Field "bits"] (RegVal_Struct [("bits", RegVal_Base (Val_Symbolic 126%Z))]) Mk_annot :t:
+            WriteReg "PC" [] (RegVal_Base (Val_Symbolic 12%Z)) Mk_annot :t:
             tnil;
-            Smt (Assert (Unop (Not) (Val (Val_Symbolic 111%Z) Mk_annot) Mk_annot)) Mk_annot :t:
-            Smt (DefineConst 129%Z (Manyop (Bvmanyarith Bvand) [Manyop (Bvmanyarith Bvor) [Manyop (Bvmanyarith Bvand) [Manyop (Bvmanyarith Bvor) [Manyop (Bvmanyarith Bvand) [Manyop (Bvmanyarith Bvand) [Val (Val_Symbolic 24%Z) Mk_annot; Val (Val_Bits (BV 64%N 0x7fffffffffffffff%Z)) Mk_annot] Mk_annot; Val (Val_Bits (BV 64%N 0xfffffff3ffffffff%Z)) Mk_annot] Mk_annot; Binop ((Bvarith Bvshl)) (Unop (ZeroExtend 62%N) (Unop (Extract 35%N 34%N) (Val (Val_Symbolic 14%Z) Mk_annot) Mk_annot) Mk_annot) (Val (Val_Bits (BV 64%N 0x22%Z)) Mk_annot) Mk_annot] Mk_annot; Val (Val_Bits (BV 64%N 0xfffffffcffffffff%Z)) Mk_annot] Mk_annot; Binop ((Bvarith Bvshl)) (Unop (ZeroExtend 62%N) (Unop (Extract 33%N 32%N) (Val (Val_Symbolic 14%Z) Mk_annot) Mk_annot) Mk_annot) (Val (Val_Bits (BV 64%N 0x20%Z)) Mk_annot) Mk_annot] Mk_annot; Val (Val_Bits (BV 64%N 0xffffffcfffffffff%Z)) Mk_annot] Mk_annot)) Mk_annot :t:
+            Smt (Assert (Unop (Not) (Val (Val_Symbolic 120%Z) Mk_annot) Mk_annot)) Mk_annot :t:
+            Smt (DefineConst 138%Z (Manyop (Bvmanyarith Bvand) [Manyop (Bvmanyarith Bvor) [Manyop (Bvmanyarith Bvand) [Manyop (Bvmanyarith Bvor) [Manyop (Bvmanyarith Bvand) [Manyop (Bvmanyarith Bvand) [Val (Val_Symbolic 33%Z) Mk_annot; Val (Val_Bits (BV 64%N 0x7fffffffffffffff%Z)) Mk_annot] Mk_annot; Val (Val_Bits (BV 64%N 0xfffffff3ffffffff%Z)) Mk_annot] Mk_annot; Binop ((Bvarith Bvshl)) (Unop (ZeroExtend 62%N) (Unop (Extract 35%N 34%N) (Val (Val_Symbolic 23%Z) Mk_annot) Mk_annot) Mk_annot) (Val (Val_Bits (BV 64%N 0x22%Z)) Mk_annot) Mk_annot] Mk_annot; Val (Val_Bits (BV 64%N 0xfffffffcffffffff%Z)) Mk_annot] Mk_annot; Binop ((Bvarith Bvshl)) (Unop (ZeroExtend 62%N) (Unop (Extract 33%N 32%N) (Val (Val_Symbolic 23%Z) Mk_annot) Mk_annot) Mk_annot) (Val (Val_Bits (BV 64%N 0x20%Z)) Mk_annot) Mk_annot] Mk_annot; Val (Val_Bits (BV 64%N 0xffffffcfffffffff%Z)) Mk_annot] Mk_annot)) Mk_annot :t:
             ReadReg "misa" [Field "bits"] (RegVal_Struct [("bits", RegVal_Base (Val_Symbolic 1%Z))]) Mk_annot :t:
-            WriteReg "mstatus" [Field "bits"] (RegVal_Struct [("bits", RegVal_Base (Val_Symbolic 129%Z))]) Mk_annot :t:
-            ReadReg "mstatus" [Field "bits"] (RegVal_Struct [("bits", RegVal_Base (Val_Symbolic 129%Z))]) Mk_annot :t:
-            WriteReg "PC" [] (RegVal_Base (Val_Symbolic 3%Z)) Mk_annot :t:
+            WriteReg "mstatus" [Field "bits"] (RegVal_Struct [("bits", RegVal_Base (Val_Symbolic 138%Z))]) Mk_annot :t:
+            ReadReg "mstatus" [Field "bits"] (RegVal_Struct [("bits", RegVal_Base (Val_Symbolic 138%Z))]) Mk_annot :t:
+            WriteReg "PC" [] (RegVal_Base (Val_Symbolic 12%Z)) Mk_annot :t:
             tnil
           ];
-          Smt (Assert (Unop (Not) (Val (Val_Symbolic 109%Z) Mk_annot) Mk_annot)) Mk_annot :t:
-          Smt (DefineConst 141%Z (Manyop (Bvmanyarith Bvand) [Manyop (Bvmanyarith Bvor) [Manyop (Bvmanyarith Bvand) [Manyop (Bvmanyarith Bvor) [Manyop (Bvmanyarith Bvand) [Manyop (Bvmanyarith Bvand) [Val (Val_Symbolic 24%Z) Mk_annot; Val (Val_Bits (BV 64%N 0x7fffffffffffffff%Z)) Mk_annot] Mk_annot; Val (Val_Bits (BV 64%N 0xfffffff3ffffffff%Z)) Mk_annot] Mk_annot; Binop ((Bvarith Bvshl)) (Unop (ZeroExtend 62%N) (Unop (Extract 35%N 34%N) (Val (Val_Symbolic 14%Z) Mk_annot) Mk_annot) Mk_annot) (Val (Val_Bits (BV 64%N 0x22%Z)) Mk_annot) Mk_annot] Mk_annot; Val (Val_Bits (BV 64%N 0xfffffffcffffffff%Z)) Mk_annot] Mk_annot; Binop ((Bvarith Bvshl)) (Unop (ZeroExtend 62%N) (Unop (Extract 33%N 32%N) (Val (Val_Symbolic 14%Z) Mk_annot) Mk_annot) Mk_annot) (Val (Val_Bits (BV 64%N 0x20%Z)) Mk_annot) Mk_annot] Mk_annot; Val (Val_Bits (BV 64%N 0xffffffcfffffffff%Z)) Mk_annot] Mk_annot)) Mk_annot :t:
+          Smt (Assert (Unop (Not) (Val (Val_Symbolic 118%Z) Mk_annot) Mk_annot)) Mk_annot :t:
+          Smt (DefineConst 150%Z (Manyop (Bvmanyarith Bvand) [Manyop (Bvmanyarith Bvor) [Manyop (Bvmanyarith Bvand) [Manyop (Bvmanyarith Bvor) [Manyop (Bvmanyarith Bvand) [Manyop (Bvmanyarith Bvand) [Val (Val_Symbolic 33%Z) Mk_annot; Val (Val_Bits (BV 64%N 0x7fffffffffffffff%Z)) Mk_annot] Mk_annot; Val (Val_Bits (BV 64%N 0xfffffff3ffffffff%Z)) Mk_annot] Mk_annot; Binop ((Bvarith Bvshl)) (Unop (ZeroExtend 62%N) (Unop (Extract 35%N 34%N) (Val (Val_Symbolic 23%Z) Mk_annot) Mk_annot) Mk_annot) (Val (Val_Bits (BV 64%N 0x22%Z)) Mk_annot) Mk_annot] Mk_annot; Val (Val_Bits (BV 64%N 0xfffffffcffffffff%Z)) Mk_annot] Mk_annot; Binop ((Bvarith Bvshl)) (Unop (ZeroExtend 62%N) (Unop (Extract 33%N 32%N) (Val (Val_Symbolic 23%Z) Mk_annot) Mk_annot) Mk_annot) (Val (Val_Bits (BV 64%N 0x20%Z)) Mk_annot) Mk_annot] Mk_annot; Val (Val_Bits (BV 64%N 0xffffffcfffffffff%Z)) Mk_annot] Mk_annot)) Mk_annot :t:
           ReadReg "misa" [Field "bits"] (RegVal_Struct [("bits", RegVal_Base (Val_Symbolic 1%Z))]) Mk_annot :t:
-          WriteReg "mstatus" [Field "bits"] (RegVal_Struct [("bits", RegVal_Base (Val_Symbolic 141%Z))]) Mk_annot :t:
-          ReadReg "mstatus" [Field "bits"] (RegVal_Struct [("bits", RegVal_Base (Val_Symbolic 141%Z))]) Mk_annot :t:
-          WriteReg "PC" [] (RegVal_Base (Val_Symbolic 3%Z)) Mk_annot :t:
+          WriteReg "mstatus" [Field "bits"] (RegVal_Struct [("bits", RegVal_Base (Val_Symbolic 150%Z))]) Mk_annot :t:
+          ReadReg "mstatus" [Field "bits"] (RegVal_Struct [("bits", RegVal_Base (Val_Symbolic 150%Z))]) Mk_annot :t:
+          WriteReg "PC" [] (RegVal_Base (Val_Symbolic 12%Z)) Mk_annot :t:
           tnil
         ];
-        Smt (Assert (Unop (Not) (Val (Val_Symbolic 107%Z) Mk_annot) Mk_annot)) Mk_annot :t:
-        Smt (DefineConst 153%Z (Manyop (Bvmanyarith Bvand) [Manyop (Bvmanyarith Bvor) [Manyop (Bvmanyarith Bvand) [Manyop (Bvmanyarith Bvor) [Manyop (Bvmanyarith Bvand) [Manyop (Bvmanyarith Bvand) [Val (Val_Symbolic 24%Z) Mk_annot; Val (Val_Bits (BV 64%N 0x7fffffffffffffff%Z)) Mk_annot] Mk_annot; Val (Val_Bits (BV 64%N 0xfffffff3ffffffff%Z)) Mk_annot] Mk_annot; Binop ((Bvarith Bvshl)) (Unop (ZeroExtend 62%N) (Unop (Extract 35%N 34%N) (Val (Val_Symbolic 14%Z) Mk_annot) Mk_annot) Mk_annot) (Val (Val_Bits (BV 64%N 0x22%Z)) Mk_annot) Mk_annot] Mk_annot; Val (Val_Bits (BV 64%N 0xfffffffcffffffff%Z)) Mk_annot] Mk_annot; Binop ((Bvarith Bvshl)) (Unop (ZeroExtend 62%N) (Unop (Extract 33%N 32%N) (Val (Val_Symbolic 14%Z) Mk_annot) Mk_annot) Mk_annot) (Val (Val_Bits (BV 64%N 0x20%Z)) Mk_annot) Mk_annot] Mk_annot; Val (Val_Bits (BV 64%N 0xffffffcfffffffff%Z)) Mk_annot] Mk_annot)) Mk_annot :t:
+        Smt (Assert (Unop (Not) (Val (Val_Symbolic 116%Z) Mk_annot) Mk_annot)) Mk_annot :t:
+        Smt (DefineConst 162%Z (Manyop (Bvmanyarith Bvand) [Manyop (Bvmanyarith Bvor) [Manyop (Bvmanyarith Bvand) [Manyop (Bvmanyarith Bvor) [Manyop (Bvmanyarith Bvand) [Manyop (Bvmanyarith Bvand) [Val (Val_Symbolic 33%Z) Mk_annot; Val (Val_Bits (BV 64%N 0x7fffffffffffffff%Z)) Mk_annot] Mk_annot; Val (Val_Bits (BV 64%N 0xfffffff3ffffffff%Z)) Mk_annot] Mk_annot; Binop ((Bvarith Bvshl)) (Unop (ZeroExtend 62%N) (Unop (Extract 35%N 34%N) (Val (Val_Symbolic 23%Z) Mk_annot) Mk_annot) Mk_annot) (Val (Val_Bits (BV 64%N 0x22%Z)) Mk_annot) Mk_annot] Mk_annot; Val (Val_Bits (BV 64%N 0xfffffffcffffffff%Z)) Mk_annot] Mk_annot; Binop ((Bvarith Bvshl)) (Unop (ZeroExtend 62%N) (Unop (Extract 33%N 32%N) (Val (Val_Symbolic 23%Z) Mk_annot) Mk_annot) Mk_annot) (Val (Val_Bits (BV 64%N 0x20%Z)) Mk_annot) Mk_annot] Mk_annot; Val (Val_Bits (BV 64%N 0xffffffcfffffffff%Z)) Mk_annot] Mk_annot)) Mk_annot :t:
         ReadReg "misa" [Field "bits"] (RegVal_Struct [("bits", RegVal_Base (Val_Symbolic 1%Z))]) Mk_annot :t:
-        WriteReg "mstatus" [Field "bits"] (RegVal_Struct [("bits", RegVal_Base (Val_Symbolic 153%Z))]) Mk_annot :t:
-        ReadReg "mstatus" [Field "bits"] (RegVal_Struct [("bits", RegVal_Base (Val_Symbolic 153%Z))]) Mk_annot :t:
-        WriteReg "PC" [] (RegVal_Base (Val_Symbolic 3%Z)) Mk_annot :t:
+        WriteReg "mstatus" [Field "bits"] (RegVal_Struct [("bits", RegVal_Base (Val_Symbolic 162%Z))]) Mk_annot :t:
+        ReadReg "mstatus" [Field "bits"] (RegVal_Struct [("bits", RegVal_Base (Val_Symbolic 162%Z))]) Mk_annot :t:
+        WriteReg "PC" [] (RegVal_Base (Val_Symbolic 12%Z)) Mk_annot :t:
         tnil
       ]
     ];
-    Smt (Assert (Unop (Not) (Val (Val_Symbolic 27%Z) Mk_annot) Mk_annot)) Mk_annot :t:
-    Smt (DefineConst 163%Z (Unop (Extract 10%N 9%N) (Val (Val_Symbolic 24%Z) Mk_annot) Mk_annot)) Mk_annot :t:
-    Smt (DefineConst 165%Z (Unop (Not) (Binop (Eq) (Val (Val_Symbolic 163%Z) Mk_annot) (Val (Val_Bits (BV 2%N 0x0%Z)) Mk_annot) Mk_annot) Mk_annot)) Mk_annot :t:
+    Smt (Assert (Unop (Not) (Val (Val_Symbolic 36%Z) Mk_annot) Mk_annot)) Mk_annot :t:
+    Smt (DefineConst 172%Z (Unop (Extract 10%N 9%N) (Val (Val_Symbolic 33%Z) Mk_annot) Mk_annot)) Mk_annot :t:
+    Smt (DefineConst 174%Z (Unop (Not) (Binop (Eq) (Val (Val_Symbolic 172%Z) Mk_annot) (Val (Val_Bits (BV 2%N 0x0%Z)) Mk_annot) Mk_annot) Mk_annot)) Mk_annot :t:
     tcases [
-      Smt (Assert (Val (Val_Symbolic 165%Z) Mk_annot)) Mk_annot :t:
-      Smt (DefineConst 167%Z (Unop (Not) (Binop (Eq) (Val (Val_Symbolic 163%Z) Mk_annot) (Val (Val_Bits (BV 2%N 0x1%Z)) Mk_annot) Mk_annot) Mk_annot)) Mk_annot :t:
+      Smt (Assert (Val (Val_Symbolic 174%Z) Mk_annot)) Mk_annot :t:
+      Smt (DefineConst 176%Z (Unop (Not) (Binop (Eq) (Val (Val_Symbolic 172%Z) Mk_annot) (Val (Val_Bits (BV 2%N 0x1%Z)) Mk_annot) Mk_annot) Mk_annot)) Mk_annot :t:
       tcases [
-        Smt (Assert (Val (Val_Symbolic 167%Z) Mk_annot)) Mk_annot :t:
-        Smt (DefineConst 169%Z (Unop (Not) (Binop (Eq) (Val (Val_Symbolic 163%Z) Mk_annot) (Val (Val_Bits (BV 2%N 0x2%Z)) Mk_annot) Mk_annot) Mk_annot)) Mk_annot :t:
+        Smt (Assert (Val (Val_Symbolic 176%Z) Mk_annot)) Mk_annot :t:
+        Smt (DefineConst 178%Z (Unop (Not) (Binop (Eq) (Val (Val_Symbolic 172%Z) Mk_annot) (Val (Val_Bits (BV 2%N 0x2%Z)) Mk_annot) Mk_annot) Mk_annot)) Mk_annot :t:
         tcases [
-          Smt (Assert (Val (Val_Symbolic 169%Z) Mk_annot)) Mk_annot :t:
-          Smt (DefineConst 175%Z (Manyop (Bvmanyarith Bvand) [Manyop (Bvmanyarith Bvor) [Manyop (Bvmanyarith Bvand) [Manyop (Bvmanyarith Bvor) [Manyop (Bvmanyarith Bvand) [Manyop (Bvmanyarith Bvor) [Manyop (Bvmanyarith Bvand) [Val (Val_Symbolic 24%Z) Mk_annot; Val (Val_Bits (BV 64%N 0x7fffffffffffffff%Z)) Mk_annot] Mk_annot; Val (Val_Bits (BV 64%N 0x8000000000000000%Z)) Mk_annot] Mk_annot; Val (Val_Bits (BV 64%N 0xfffffff3ffffffff%Z)) Mk_annot] Mk_annot; Binop ((Bvarith Bvshl)) (Unop (ZeroExtend 62%N) (Unop (Extract 35%N 34%N) (Val (Val_Symbolic 14%Z) Mk_annot) Mk_annot) Mk_annot) (Val (Val_Bits (BV 64%N 0x22%Z)) Mk_annot) Mk_annot] Mk_annot; Val (Val_Bits (BV 64%N 0xfffffffcffffffff%Z)) Mk_annot] Mk_annot; Binop ((Bvarith Bvshl)) (Unop (ZeroExtend 62%N) (Unop (Extract 33%N 32%N) (Val (Val_Symbolic 14%Z) Mk_annot) Mk_annot) Mk_annot) (Val (Val_Bits (BV 64%N 0x20%Z)) Mk_annot) Mk_annot] Mk_annot; Val (Val_Bits (BV 64%N 0xffffffcfffffffff%Z)) Mk_annot] Mk_annot)) Mk_annot :t:
+          Smt (Assert (Val (Val_Symbolic 178%Z) Mk_annot)) Mk_annot :t:
+          Smt (DefineConst 184%Z (Manyop (Bvmanyarith Bvand) [Manyop (Bvmanyarith Bvor) [Manyop (Bvmanyarith Bvand) [Manyop (Bvmanyarith Bvor) [Manyop (Bvmanyarith Bvand) [Manyop (Bvmanyarith Bvor) [Manyop (Bvmanyarith Bvand) [Val (Val_Symbolic 33%Z) Mk_annot; Val (Val_Bits (BV 64%N 0x7fffffffffffffff%Z)) Mk_annot] Mk_annot; Val (Val_Bits (BV 64%N 0x8000000000000000%Z)) Mk_annot] Mk_annot; Val (Val_Bits (BV 64%N 0xfffffff3ffffffff%Z)) Mk_annot] Mk_annot; Binop ((Bvarith Bvshl)) (Unop (ZeroExtend 62%N) (Unop (Extract 35%N 34%N) (Val (Val_Symbolic 23%Z) Mk_annot) Mk_annot) Mk_annot) (Val (Val_Bits (BV 64%N 0x22%Z)) Mk_annot) Mk_annot] Mk_annot; Val (Val_Bits (BV 64%N 0xfffffffcffffffff%Z)) Mk_annot] Mk_annot; Binop ((Bvarith Bvshl)) (Unop (ZeroExtend 62%N) (Unop (Extract 33%N 32%N) (Val (Val_Symbolic 23%Z) Mk_annot) Mk_annot) Mk_annot) (Val (Val_Bits (BV 64%N 0x20%Z)) Mk_annot) Mk_annot] Mk_annot; Val (Val_Bits (BV 64%N 0xffffffcfffffffff%Z)) Mk_annot] Mk_annot)) Mk_annot :t:
           ReadReg "misa" [Field "bits"] (RegVal_Struct [("bits", RegVal_Base (Val_Symbolic 1%Z))]) Mk_annot :t:
-          WriteReg "mstatus" [Field "bits"] (RegVal_Struct [("bits", RegVal_Base (Val_Symbolic 175%Z))]) Mk_annot :t:
-          ReadReg "mstatus" [Field "bits"] (RegVal_Struct [("bits", RegVal_Base (Val_Symbolic 175%Z))]) Mk_annot :t:
-          WriteReg "PC" [] (RegVal_Base (Val_Symbolic 3%Z)) Mk_annot :t:
+          WriteReg "mstatus" [Field "bits"] (RegVal_Struct [("bits", RegVal_Base (Val_Symbolic 184%Z))]) Mk_annot :t:
+          ReadReg "mstatus" [Field "bits"] (RegVal_Struct [("bits", RegVal_Base (Val_Symbolic 184%Z))]) Mk_annot :t:
+          WriteReg "PC" [] (RegVal_Base (Val_Symbolic 12%Z)) Mk_annot :t:
           tnil;
-          Smt (Assert (Unop (Not) (Val (Val_Symbolic 169%Z) Mk_annot) Mk_annot)) Mk_annot :t:
-          Smt (DefineConst 187%Z (Manyop (Bvmanyarith Bvand) [Manyop (Bvmanyarith Bvor) [Manyop (Bvmanyarith Bvand) [Manyop (Bvmanyarith Bvor) [Manyop (Bvmanyarith Bvand) [Manyop (Bvmanyarith Bvand) [Val (Val_Symbolic 24%Z) Mk_annot; Val (Val_Bits (BV 64%N 0x7fffffffffffffff%Z)) Mk_annot] Mk_annot; Val (Val_Bits (BV 64%N 0xfffffff3ffffffff%Z)) Mk_annot] Mk_annot; Binop ((Bvarith Bvshl)) (Unop (ZeroExtend 62%N) (Unop (Extract 35%N 34%N) (Val (Val_Symbolic 14%Z) Mk_annot) Mk_annot) Mk_annot) (Val (Val_Bits (BV 64%N 0x22%Z)) Mk_annot) Mk_annot] Mk_annot; Val (Val_Bits (BV 64%N 0xfffffffcffffffff%Z)) Mk_annot] Mk_annot; Binop ((Bvarith Bvshl)) (Unop (ZeroExtend 62%N) (Unop (Extract 33%N 32%N) (Val (Val_Symbolic 14%Z) Mk_annot) Mk_annot) Mk_annot) (Val (Val_Bits (BV 64%N 0x20%Z)) Mk_annot) Mk_annot] Mk_annot; Val (Val_Bits (BV 64%N 0xffffffcfffffffff%Z)) Mk_annot] Mk_annot)) Mk_annot :t:
+          Smt (Assert (Unop (Not) (Val (Val_Symbolic 178%Z) Mk_annot) Mk_annot)) Mk_annot :t:
+          Smt (DefineConst 196%Z (Manyop (Bvmanyarith Bvand) [Manyop (Bvmanyarith Bvor) [Manyop (Bvmanyarith Bvand) [Manyop (Bvmanyarith Bvor) [Manyop (Bvmanyarith Bvand) [Manyop (Bvmanyarith Bvand) [Val (Val_Symbolic 33%Z) Mk_annot; Val (Val_Bits (BV 64%N 0x7fffffffffffffff%Z)) Mk_annot] Mk_annot; Val (Val_Bits (BV 64%N 0xfffffff3ffffffff%Z)) Mk_annot] Mk_annot; Binop ((Bvarith Bvshl)) (Unop (ZeroExtend 62%N) (Unop (Extract 35%N 34%N) (Val (Val_Symbolic 23%Z) Mk_annot) Mk_annot) Mk_annot) (Val (Val_Bits (BV 64%N 0x22%Z)) Mk_annot) Mk_annot] Mk_annot; Val (Val_Bits (BV 64%N 0xfffffffcffffffff%Z)) Mk_annot] Mk_annot; Binop ((Bvarith Bvshl)) (Unop (ZeroExtend 62%N) (Unop (Extract 33%N 32%N) (Val (Val_Symbolic 23%Z) Mk_annot) Mk_annot) Mk_annot) (Val (Val_Bits (BV 64%N 0x20%Z)) Mk_annot) Mk_annot] Mk_annot; Val (Val_Bits (BV 64%N 0xffffffcfffffffff%Z)) Mk_annot] Mk_annot)) Mk_annot :t:
           ReadReg "misa" [Field "bits"] (RegVal_Struct [("bits", RegVal_Base (Val_Symbolic 1%Z))]) Mk_annot :t:
-          WriteReg "mstatus" [Field "bits"] (RegVal_Struct [("bits", RegVal_Base (Val_Symbolic 187%Z))]) Mk_annot :t:
-          ReadReg "mstatus" [Field "bits"] (RegVal_Struct [("bits", RegVal_Base (Val_Symbolic 187%Z))]) Mk_annot :t:
-          WriteReg "PC" [] (RegVal_Base (Val_Symbolic 3%Z)) Mk_annot :t:
+          WriteReg "mstatus" [Field "bits"] (RegVal_Struct [("bits", RegVal_Base (Val_Symbolic 196%Z))]) Mk_annot :t:
+          ReadReg "mstatus" [Field "bits"] (RegVal_Struct [("bits", RegVal_Base (Val_Symbolic 196%Z))]) Mk_annot :t:
+          WriteReg "PC" [] (RegVal_Base (Val_Symbolic 12%Z)) Mk_annot :t:
           tnil
         ];
-        Smt (Assert (Unop (Not) (Val (Val_Symbolic 167%Z) Mk_annot) Mk_annot)) Mk_annot :t:
-        Smt (DefineConst 199%Z (Manyop (Bvmanyarith Bvand) [Manyop (Bvmanyarith Bvor) [Manyop (Bvmanyarith Bvand) [Manyop (Bvmanyarith Bvor) [Manyop (Bvmanyarith Bvand) [Manyop (Bvmanyarith Bvand) [Val (Val_Symbolic 24%Z) Mk_annot; Val (Val_Bits (BV 64%N 0x7fffffffffffffff%Z)) Mk_annot] Mk_annot; Val (Val_Bits (BV 64%N 0xfffffff3ffffffff%Z)) Mk_annot] Mk_annot; Binop ((Bvarith Bvshl)) (Unop (ZeroExtend 62%N) (Unop (Extract 35%N 34%N) (Val (Val_Symbolic 14%Z) Mk_annot) Mk_annot) Mk_annot) (Val (Val_Bits (BV 64%N 0x22%Z)) Mk_annot) Mk_annot] Mk_annot; Val (Val_Bits (BV 64%N 0xfffffffcffffffff%Z)) Mk_annot] Mk_annot; Binop ((Bvarith Bvshl)) (Unop (ZeroExtend 62%N) (Unop (Extract 33%N 32%N) (Val (Val_Symbolic 14%Z) Mk_annot) Mk_annot) Mk_annot) (Val (Val_Bits (BV 64%N 0x20%Z)) Mk_annot) Mk_annot] Mk_annot; Val (Val_Bits (BV 64%N 0xffffffcfffffffff%Z)) Mk_annot] Mk_annot)) Mk_annot :t:
+        Smt (Assert (Unop (Not) (Val (Val_Symbolic 176%Z) Mk_annot) Mk_annot)) Mk_annot :t:
+        Smt (DefineConst 208%Z (Manyop (Bvmanyarith Bvand) [Manyop (Bvmanyarith Bvor) [Manyop (Bvmanyarith Bvand) [Manyop (Bvmanyarith Bvor) [Manyop (Bvmanyarith Bvand) [Manyop (Bvmanyarith Bvand) [Val (Val_Symbolic 33%Z) Mk_annot; Val (Val_Bits (BV 64%N 0x7fffffffffffffff%Z)) Mk_annot] Mk_annot; Val (Val_Bits (BV 64%N 0xfffffff3ffffffff%Z)) Mk_annot] Mk_annot; Binop ((Bvarith Bvshl)) (Unop (ZeroExtend 62%N) (Unop (Extract 35%N 34%N) (Val (Val_Symbolic 23%Z) Mk_annot) Mk_annot) Mk_annot) (Val (Val_Bits (BV 64%N 0x22%Z)) Mk_annot) Mk_annot] Mk_annot; Val (Val_Bits (BV 64%N 0xfffffffcffffffff%Z)) Mk_annot] Mk_annot; Binop ((Bvarith Bvshl)) (Unop (ZeroExtend 62%N) (Unop (Extract 33%N 32%N) (Val (Val_Symbolic 23%Z) Mk_annot) Mk_annot) Mk_annot) (Val (Val_Bits (BV 64%N 0x20%Z)) Mk_annot) Mk_annot] Mk_annot; Val (Val_Bits (BV 64%N 0xffffffcfffffffff%Z)) Mk_annot] Mk_annot)) Mk_annot :t:
         ReadReg "misa" [Field "bits"] (RegVal_Struct [("bits", RegVal_Base (Val_Symbolic 1%Z))]) Mk_annot :t:
-        WriteReg "mstatus" [Field "bits"] (RegVal_Struct [("bits", RegVal_Base (Val_Symbolic 199%Z))]) Mk_annot :t:
-        ReadReg "mstatus" [Field "bits"] (RegVal_Struct [("bits", RegVal_Base (Val_Symbolic 199%Z))]) Mk_annot :t:
-        WriteReg "PC" [] (RegVal_Base (Val_Symbolic 3%Z)) Mk_annot :t:
+        WriteReg "mstatus" [Field "bits"] (RegVal_Struct [("bits", RegVal_Base (Val_Symbolic 208%Z))]) Mk_annot :t:
+        ReadReg "mstatus" [Field "bits"] (RegVal_Struct [("bits", RegVal_Base (Val_Symbolic 208%Z))]) Mk_annot :t:
+        WriteReg "PC" [] (RegVal_Base (Val_Symbolic 12%Z)) Mk_annot :t:
         tnil
       ];
-      Smt (Assert (Unop (Not) (Val (Val_Symbolic 165%Z) Mk_annot) Mk_annot)) Mk_annot :t:
-      Smt (DefineConst 211%Z (Manyop (Bvmanyarith Bvand) [Manyop (Bvmanyarith Bvor) [Manyop (Bvmanyarith Bvand) [Manyop (Bvmanyarith Bvor) [Manyop (Bvmanyarith Bvand) [Manyop (Bvmanyarith Bvand) [Val (Val_Symbolic 24%Z) Mk_annot; Val (Val_Bits (BV 64%N 0x7fffffffffffffff%Z)) Mk_annot] Mk_annot; Val (Val_Bits (BV 64%N 0xfffffff3ffffffff%Z)) Mk_annot] Mk_annot; Binop ((Bvarith Bvshl)) (Unop (ZeroExtend 62%N) (Unop (Extract 35%N 34%N) (Val (Val_Symbolic 14%Z) Mk_annot) Mk_annot) Mk_annot) (Val (Val_Bits (BV 64%N 0x22%Z)) Mk_annot) Mk_annot] Mk_annot; Val (Val_Bits (BV 64%N 0xfffffffcffffffff%Z)) Mk_annot] Mk_annot; Binop ((Bvarith Bvshl)) (Unop (ZeroExtend 62%N) (Unop (Extract 33%N 32%N) (Val (Val_Symbolic 14%Z) Mk_annot) Mk_annot) Mk_annot) (Val (Val_Bits (BV 64%N 0x20%Z)) Mk_annot) Mk_annot] Mk_annot; Val (Val_Bits (BV 64%N 0xffffffcfffffffff%Z)) Mk_annot] Mk_annot)) Mk_annot :t:
+      Smt (Assert (Unop (Not) (Val (Val_Symbolic 174%Z) Mk_annot) Mk_annot)) Mk_annot :t:
+      Smt (DefineConst 220%Z (Manyop (Bvmanyarith Bvand) [Manyop (Bvmanyarith Bvor) [Manyop (Bvmanyarith Bvand) [Manyop (Bvmanyarith Bvor) [Manyop (Bvmanyarith Bvand) [Manyop (Bvmanyarith Bvand) [Val (Val_Symbolic 33%Z) Mk_annot; Val (Val_Bits (BV 64%N 0x7fffffffffffffff%Z)) Mk_annot] Mk_annot; Val (Val_Bits (BV 64%N 0xfffffff3ffffffff%Z)) Mk_annot] Mk_annot; Binop ((Bvarith Bvshl)) (Unop (ZeroExtend 62%N) (Unop (Extract 35%N 34%N) (Val (Val_Symbolic 23%Z) Mk_annot) Mk_annot) Mk_annot) (Val (Val_Bits (BV 64%N 0x22%Z)) Mk_annot) Mk_annot] Mk_annot; Val (Val_Bits (BV 64%N 0xfffffffcffffffff%Z)) Mk_annot] Mk_annot; Binop ((Bvarith Bvshl)) (Unop (ZeroExtend 62%N) (Unop (Extract 33%N 32%N) (Val (Val_Symbolic 23%Z) Mk_annot) Mk_annot) Mk_annot) (Val (Val_Bits (BV 64%N 0x20%Z)) Mk_annot) Mk_annot] Mk_annot; Val (Val_Bits (BV 64%N 0xffffffcfffffffff%Z)) Mk_annot] Mk_annot)) Mk_annot :t:
       ReadReg "misa" [Field "bits"] (RegVal_Struct [("bits", RegVal_Base (Val_Symbolic 1%Z))]) Mk_annot :t:
-      WriteReg "mstatus" [Field "bits"] (RegVal_Struct [("bits", RegVal_Base (Val_Symbolic 211%Z))]) Mk_annot :t:
-      ReadReg "mstatus" [Field "bits"] (RegVal_Struct [("bits", RegVal_Base (Val_Symbolic 211%Z))]) Mk_annot :t:
-      WriteReg "PC" [] (RegVal_Base (Val_Symbolic 3%Z)) Mk_annot :t:
+      WriteReg "mstatus" [Field "bits"] (RegVal_Struct [("bits", RegVal_Base (Val_Symbolic 220%Z))]) Mk_annot :t:
+      ReadReg "mstatus" [Field "bits"] (RegVal_Struct [("bits", RegVal_Base (Val_Symbolic 220%Z))]) Mk_annot :t:
+      WriteReg "PC" [] (RegVal_Base (Val_Symbolic 12%Z)) Mk_annot :t:
       tnil
     ]
   ]
