dorami/instructions/Sally_Port/a1c.v
@@ -1,13 +1,31 @@
 From isla Require Import opsem.
 
 Definition a1c : isla_trace :=
-  Smt (DeclareConst 0%Z (Ty_BitVec 64%N)) Mk_annot :t:
-  ReadReg "PC" [] (RegVal_Base (Val_Symbolic 0%Z)) Mk_annot :t:
-  Smt (DefineConst 1%Z (Manyop (Bvmanyarith Bvadd) [Val (Val_Symbolic 0%Z) Mk_annot; Val (Val_Bits (BV 64%N 0x4%Z)) Mk_annot] Mk_annot)) Mk_annot :t:
-  Smt (DeclareConst 2%Z (Ty_BitVec 64%N)) Mk_annot :t:
-  ReadReg "x5" [] (RegVal_Base (Val_Symbolic 2%Z)) Mk_annot :t:
-  Smt (DefineConst 5%Z (Unop (SignExtend 32%N) (Manyop (Bvmanyarith Bvadd) [Val (Val_Bits (BV 32%N 0xfffffc4f%Z)) Mk_annot; Unop (Extract 31%N 0%N) (Val (Val_Symbolic 2%Z) Mk_annot) Mk_annot] Mk_annot) Mk_annot)) Mk_annot :t:
-  WriteReg "x5" [] (RegVal_Base (Val_Symbolic 5%Z)) Mk_annot :t:
-  WriteReg "PC" [] (RegVal_Base (Val_Symbolic 1%Z)) Mk_annot :t:
+  Smt (DeclareConst 0%Z (Ty_BitVec 8%N)) Mk_annot :t:
+  Assume (AExp_Binop (Eq) (AExp_Val (AVal_Var "pmp0cfg" [Field "bits"]) Mk_annot) (AExp_Val (AVal_Bits (BV 8%N 0x0%Z)) Mk_annot) Mk_annot) Mk_annot :t:
+  Smt (DeclareConst 1%Z (Ty_BitVec 8%N)) Mk_annot :t:
+  Assume (AExp_Binop (Eq) (AExp_Val (AVal_Var "pmp1cfg" [Field "bits"]) Mk_annot) (AExp_Val (AVal_Bits (BV 8%N 0x0%Z)) Mk_annot) Mk_annot) Mk_annot :t:
+  Smt (DeclareConst 2%Z (Ty_BitVec 8%N)) Mk_annot :t:
+  Assume (AExp_Binop (Eq) (AExp_Val (AVal_Var "pmp2cfg" [Field "bits"]) Mk_annot) (AExp_Val (AVal_Bits (BV 8%N 0x0%Z)) Mk_annot) Mk_annot) Mk_annot :t:
+  Smt (DeclareConst 3%Z (Ty_BitVec 8%N)) Mk_annot :t:
+  Assume (AExp_Binop (Eq) (AExp_Val (AVal_Var "pmp3cfg" [Field "bits"]) Mk_annot) (AExp_Val (AVal_Bits (BV 8%N 0x0%Z)) Mk_annot) Mk_annot) Mk_annot :t:
+  Smt (DeclareConst 4%Z (Ty_BitVec 8%N)) Mk_annot :t:
+  Assume (AExp_Binop (Eq) (AExp_Val (AVal_Var "pmp4cfg" [Field "bits"]) Mk_annot) (AExp_Val (AVal_Bits (BV 8%N 0x0%Z)) Mk_annot) Mk_annot) Mk_annot :t:
+  Smt (DeclareConst 5%Z (Ty_BitVec 8%N)) Mk_annot :t:
+  Assume (AExp_Binop (Eq) (AExp_Val (AVal_Var "pmp5cfg" [Field "bits"]) Mk_annot) (AExp_Val (AVal_Bits (BV 8%N 0x0%Z)) Mk_annot) Mk_annot) Mk_annot :t:
+  Smt (DeclareConst 6%Z (Ty_BitVec 8%N)) Mk_annot :t:
+  Assume (AExp_Binop (Eq) (AExp_Val (AVal_Var "pmp6cfg" [Field "bits"]) Mk_annot) (AExp_Val (AVal_Bits (BV 8%N 0x0%Z)) Mk_annot) Mk_annot) Mk_annot :t:
+  Smt (DeclareConst 7%Z (Ty_BitVec 8%N)) Mk_annot :t:
+  Assume (AExp_Binop (Eq) (AExp_Val (AVal_Var "pmp7cfg" [Field "bits"]) Mk_annot) (AExp_Val (AVal_Bits (BV 8%N 0x0%Z)) Mk_annot) Mk_annot) Mk_annot :t:
+  Smt (DeclareConst 8%Z (Ty_BitVec 64%N)) Mk_annot :t:
+  Assume (AExp_Binop (Eq) (AExp_Val (AVal_Var "mseccfg" [Field "bits"]) Mk_annot) (AExp_Val (AVal_Bits (BV 64%N 0x7%Z)) Mk_annot) Mk_annot) Mk_annot :t:
+  Smt (DeclareConst 9%Z (Ty_BitVec 64%N)) Mk_annot :t:
+  ReadReg "PC" [] (RegVal_Base (Val_Symbolic 9%Z)) Mk_annot :t:
+  Smt (DefineConst 10%Z (Manyop (Bvmanyarith Bvadd) [Val (Val_Symbolic 9%Z) Mk_annot; Val (Val_Bits (BV 64%N 0x4%Z)) Mk_annot] Mk_annot)) Mk_annot :t:
+  Smt (DeclareConst 11%Z (Ty_BitVec 64%N)) Mk_annot :t:
+  ReadReg "x5" [] (RegVal_Base (Val_Symbolic 11%Z)) Mk_annot :t:
+  Smt (DefineConst 12%Z (Manyop (Bvmanyarith Bvadd) [Val (Val_Symbolic 11%Z) Mk_annot; Val (Val_Bits (BV 64%N 0xfffffffffffffcc5%Z)) Mk_annot] Mk_annot)) Mk_annot :t:
+  WriteReg "x5" [] (RegVal_Base (Val_Symbolic 12%Z)) Mk_annot :t:
+  WriteReg "PC" [] (RegVal_Base (Val_Symbolic 10%Z)) Mk_annot :t:
   tnil
 .
