dorami/instructions/Sally_Port/a2c.v
@@ -1,13 +1,32 @@
 From isla Require Import opsem.
 
 Definition a2c : isla_trace :=
-  Smt (DeclareConst 0%Z (Ty_BitVec 64%N)) Mk_annot :t:
-  ReadReg "PC" [] (RegVal_Base (Val_Symbolic 0%Z)) Mk_annot :t:
-  Smt (DefineConst 1%Z (Manyop (Bvmanyarith Bvadd) [Val (Val_Symbolic 0%Z) Mk_annot; Val (Val_Bits (BV 64%N 0x4%Z)) Mk_annot] Mk_annot)) Mk_annot :t:
-  Smt (DeclareConst 2%Z (Ty_BitVec 64%N)) Mk_annot :t:
-  ReadReg "x5" [] (RegVal_Base (Val_Symbolic 2%Z)) Mk_annot :t:
-  Smt (DefineConst 3%Z (Manyop (Bvmanyarith Bvadd) [Val (Val_Symbolic 2%Z) Mk_annot; Val (Val_Bits (BV 64%N 0xfffffffffffffd1e%Z)) Mk_annot] Mk_annot)) Mk_annot :t:
-  WriteReg "x5" [] (RegVal_Base (Val_Symbolic 3%Z)) Mk_annot :t:
-  WriteReg "PC" [] (RegVal_Base (Val_Symbolic 1%Z)) Mk_annot :t:
+  Smt (DeclareConst 0%Z (Ty_BitVec 8%N)) Mk_annot :t:
+  Assume (AExp_Binop (Eq) (AExp_Val (AVal_Var "pmp0cfg" [Field "bits"]) Mk_annot) (AExp_Val (AVal_Bits (BV 8%N 0x1e%Z)) Mk_annot) Mk_annot) Mk_annot :t:
+  Smt (DeclareConst 1%Z (Ty_BitVec 8%N)) Mk_annot :t:
+  Assume (AExp_Binop (Eq) (AExp_Val (AVal_Var "pmp1cfg" [Field "bits"]) Mk_annot) (AExp_Val (AVal_Bits (BV 8%N 0x9d%Z)) Mk_annot) Mk_annot) Mk_annot :t:
+  Smt (DeclareConst 2%Z (Ty_BitVec 8%N)) Mk_annot :t:
+  Assume (AExp_Binop (Eq) (AExp_Val (AVal_Var "pmp2cfg" [Field "bits"]) Mk_annot) (AExp_Val (AVal_Bits (BV 8%N 0x98%Z)) Mk_annot) Mk_annot) Mk_annot :t:
+  Smt (DeclareConst 3%Z (Ty_BitVec 8%N)) Mk_annot :t:
+  Assume (AExp_Binop (Eq) (AExp_Val (AVal_Var "pmp3cfg" [Field "bits"]) Mk_annot) (AExp_Val (AVal_Bits (BV 8%N 0x9d%Z)) Mk_annot) Mk_annot) Mk_annot :t:
+  Smt (DeclareConst 4%Z (Ty_BitVec 8%N)) Mk_annot :t:
+  Assume (AExp_Binop (Eq) (AExp_Val (AVal_Var "pmp4cfg" [Field "bits"]) Mk_annot) (AExp_Val (AVal_Bits (BV 8%N 0x98%Z)) Mk_annot) Mk_annot) Mk_annot :t:
+  Smt (DeclareConst 5%Z (Ty_BitVec 8%N)) Mk_annot :t:
+  Assume (AExp_Binop (Eq) (AExp_Val (AVal_Var "pmp5cfg" [Field "bits"]) Mk_annot) (AExp_Val (AVal_Bits (BV 8%N 0x9b%Z)) Mk_annot) Mk_annot) Mk_annot :t:
+  Smt (DeclareConst 6%Z (Ty_BitVec 8%N)) Mk_annot :t:
+  Assume (AExp_Binop (Eq) (AExp_Val (AVal_Var "pmp6cfg" [Field "bits"]) Mk_annot) (AExp_Val (AVal_Bits (BV 8%N 0x0%Z)) Mk_annot) Mk_annot) Mk_annot :t:
+  Smt (DeclareConst 7%Z (Ty_BitVec 8%N)) Mk_annot :t:
+  Assume (AExp_Binop (Eq) (AExp_Val (AVal_Var "pmp7cfg" [Field "bits"]) Mk_annot) (AExp_Val (AVal_Bits (BV 8%N 0x0%Z)) Mk_annot) Mk_annot) Mk_annot :t:
+  Smt (DeclareConst 8%Z (Ty_BitVec 64%N)) Mk_annot :t:
+  Assume (AExp_Binop (Eq) (AExp_Val (AVal_Var "mseccfg" [Field "bits"]) Mk_annot) (AExp_Val (AVal_Bits (BV 64%N 0x7%Z)) Mk_annot) Mk_annot) Mk_annot :t:
+  Smt (DeclareConst 9%Z (Ty_BitVec 64%N)) Mk_annot :t:
+  Assume (AExp_Binop (Eq) (AExp_Val (AVal_Var "PC" []) Mk_annot) (AExp_Val (AVal_Bits (BV 64%N 0x8002102c%Z)) Mk_annot) Mk_annot) Mk_annot :t:
+  Smt (DeclareConst 10%Z (Ty_BitVec 64%N)) Mk_annot :t:
+  Assume (AExp_Binop (Eq) (AExp_Unop (Extract 2%N 2%N) (AExp_Val (AVal_Var "misa" [Field "bits"]) Mk_annot) Mk_annot) (AExp_Val (AVal_Bits (BV 1%N 0x1%Z)) Mk_annot) Mk_annot) Mk_annot :t:
+  ReadReg "PC" [] (RegVal_Base (Val_Symbolic 9%Z)) Mk_annot :t:
+  Smt (DefineConst 11%Z (Manyop (Bvmanyarith Bvadd) [Val (Val_Symbolic 9%Z) Mk_annot; Val (Val_Bits (BV 64%N 0x4%Z)) Mk_annot] Mk_annot)) Mk_annot :t:
+  Smt (DefineConst 12%Z (Manyop (Bvmanyarith Bvadd) [Val (Val_Symbolic 9%Z) Mk_annot; Val (Val_Bits (BV 64%N 0xfffffffffffdefd4%Z)) Mk_annot] Mk_annot)) Mk_annot :t:
+  Smt (DefineConst 13%Z (Unop (Extract 0%N 0%N) (Binop ((Bvarith Bvlshr)) (Val (Val_Symbolic 12%Z) Mk_annot) (Val (Val_Bits (BV 64%N 0x1%Z)) Mk_annot) Mk_annot) Mk_annot)) Mk_annot :t:
+  WriteReg "PC" [] (RegVal_Base (Val_Symbolic 12%Z)) Mk_annot :t:
   tnil
 .
