dorami/verification/SM.v
@@ -1,0 +1,194 @@
+From isla.dorami Require Import model.
+From isla.dorami Require Import transitions.
+
+Section SM.
+
+Context `{!islaG Σ} `{!threadG}.
+
+Variable csr0 : list (bv 64).
+Variable gpr0 : list (bv 64).
+Variable ret_Encl_addr : bv 64.
+
+Hypothesis csr0_length : length csr0 = 4%nat.
+Hypothesis gpr0_length : length gpr0 = 5%nat.
+
+Definition E2F_spec (mcause: bv 64) (csr gpr: list (bv 64)) (mem: bv (0x20000 * 8)) : iProp Σ :=
+  P P_mtvec P_pmpcfgs (<[2%nat := mcause]> csr) gpr mem ∗
+  instr_pre (bv_unsigned P2F_code_addr) (
+    ∃ mem', P P_mtvec P_pmpcfgs (<[2%nat := mcause]> csr0) gpr0 mem'
+  ).
+
+Arguments E2F_spec /.
+
+Definition F2E_spec (x10: bv 64) (csr gpr: list (bv 64)) (mem: bv (0x20000 * 8)): iProp Σ :=
+  P P_mtvec P_pmpcfgs csr (<[3%nat := x10]> gpr) mem ∗
+  instr_pre (bv_unsigned ret_Encl_addr) (
+    ∃ mem', P P_mtvec P_pmpcfgs csr0 (<[3%nat := x10]> gpr0) mem'
+  ).
+
+Arguments F2E_spec /.
+
+(* Save the Non-ouput and Restore the untrusted version. *)
+Hypothesis E2F : ∀ (mcause: bv 64) (csr gpr: list (bv 64)) (mem: bv (0x20000 * 8)), ⊢ instr_body (bv_unsigned P_mtvec) (E2F_spec mcause csr gpr mem).
+
+Hypothesis F2E : ∀ (x10: bv 64) (csr gpr: list (bv 64)) (mem: bv (0x20000 * 8)), ⊢ instr_body (bv_unsigned P_code_addr + P_entry_code_size) (F2E_spec x10 csr gpr mem).
+
+Definition leave_Encl mcause csr gpr Pmem Fmem :=
+  Machine P_mtvec P_pmpcfgs (<[2%nat := mcause]> csr) gpr Pmem Fmem.
+
+Arguments leave_Encl /.
+
+Definition start_F mcause Pmem Fmem :=
+  Machine F_mtvec F_pmpcfgs (<[2%nat := mcause]> csr0) (<[2%nat := (BV 64 0x989B989D981E)]> gpr0) Pmem Fmem.
+
+Arguments start_F /.
+
+Definition leave_F x10 csr gpr Pmem Fmem :=
+  Machine F_mtvec SP_pmpcfgs csr (<[3%nat := x10]> gpr) Pmem Fmem.
+
+Arguments leave_F /.
+
+Definition ret_Encl x10 Pmem Fmem :=
+  Machine P_mtvec P_pmpcfgs csr0 (<[3%nat := x10]> gpr0) Pmem Fmem.
+
+Arguments ret_Encl /.
+
+Theorem confidentiality :
+  ∀ (mcause: bv 64) (csr gpr: list (bv 64)) (Pmem: bv (0x20000 * 8)) (Fmem: bv (0x1000 * 8)),
+  length csr = 4%nat ->
+  length gpr = 5%nat ->
+  (∃ v, csr !! 0%nat = Some v ∧ (bv_extract 3 1 v) = (BV 1 0x0)) ->
+  ⊢
+  instr (bv_unsigned F_code_addr - 0x2c) (Some P2F.a0.a0) -∗
+  instr (bv_unsigned F_code_addr - 0x28) (Some P2F.a4.a4) -∗
+  instr (bv_unsigned F_code_addr - 0x24) (Some P2F.a8.a8) -∗
+  instr (bv_unsigned F_code_addr - 0x20) (Some P2F.ac.ac) -∗
+  instr (bv_unsigned F_code_addr - 0x1c) (Some P2F.a10.a10) -∗
+  instr (bv_unsigned F_code_addr - 0x18) (Some P2F.a14.a14) -∗
+  instr (bv_unsigned F_code_addr - 0x14) (Some P2F.a18.a18) -∗
+  instr (bv_unsigned F_code_addr - 0x10) (Some P2F.a1c.a1c) -∗
+  instr (bv_unsigned F_code_addr - 0xc) (Some P2F.a20.a20) -∗
+  instr (bv_unsigned F_code_addr - 0x8) (Some P2F.a24.a24) -∗
+  instr (bv_unsigned F_code_addr - 0x4) (Some P2F.a28.a28) -∗
+  instr_body (bv_unsigned P_mtvec) (
+    Machine P_mtvec P_pmpcfgs (<[2%nat := mcause]> csr) gpr Pmem Fmem ∗
+    instr_pre (bv_unsigned F_code_addr)
+      (∃ Pmem', Machine F_mtvec F_pmpcfgs (<[2%nat := mcause]> csr0) (<[2%nat := (BV 64 0x989B989D981E)]> gpr0) Pmem' Fmem)
+  ).
+Proof using E2F H csr0 csr0_length gpr0 gpr0_length ret_Encl_addr.
+  intros mcause csr gpr Pmem Fmem Hcsr Hgpr.
+  do 5 (destruct csr as [|? csr]; try inversion Hcsr).
+  do 6 (destruct gpr as [|? gpr]; try inversion Hgpr).
+  destruct csr0 as [|? csr0'] eqn:Hcsr0 ; try inversion csr0_length.
+  destruct gpr0 as [|? gpr0'] eqn:Hgpr0 ; try inversion gpr0_length.
+  do 4 (destruct csr0' as [|? csr0']; try inversion csr0_length).
+  do 5 (destruct gpr0' as [|? gpr0']; try inversion gpr0_length).
+  clear H1 H2 H3 H4 H5 H6 H7 H8 H9 H10 H11 H12 H13 H14 H15 H16 H17 H18 Hcsr Hgpr.
+  intros [ms [[= <-] Hms]].
+  iStartProof.
+  iPoseProof (E2F mcause [b; b0; mcause; b2] [b3; b4; b5; b6; b7] Pmem) as "HE2F".
+  liARun.
+  rewrite Hcsr0 Hgpr0.
+  iPoseProof (P2F [b8; b10; mcause; b12] [b9; b13; b14; b15; b16] Pmem with "[$] [$] [$] [$] [$] [$] [$] [$] [$] [$] [$]") as "HP2F"; try done.
+  liSimpl.
+  liARun.
+  iFrame.
+  Unshelve. all: prepare_sidecond.
+  all: bv_solve.
+Qed.
+
+Theorem integrity :
+  ∀ (x10: bv 64) (csr gpr: list (bv 64)) Pmem Fmem,
+  length csr = 4%nat ->
+  length gpr = 5%nat ->
+  ⊢
+  instr (bv_unsigned SP_code_addr) (Some Sally_Port.a0.a0) -∗
+  instr (bv_unsigned SP_code_addr + 0x4) (Some Sally_Port.a4.a4) -∗
+  instr (bv_unsigned SP_code_addr + 0x8) (Some Sally_Port.a8.a8) -∗
+  instr (bv_unsigned SP_code_addr + 0xc) (Some Sally_Port.ac.ac) -∗
+  instr (bv_unsigned SP_code_addr + 0x10) (Some Sally_Port.a10.a10) -∗
+  instr (bv_unsigned SP_code_addr + 0x14) (Some Sally_Port.a14.a14) -∗
+  instr (bv_unsigned SP_code_addr + 0x18) (Some Sally_Port.a18.a18) -∗
+  instr (bv_unsigned SP_code_addr + 0x1c) (Some Sally_Port.a1c.a1c) -∗
+  instr (bv_unsigned SP_code_addr + 0x20) (Some Sally_Port.a20.a20) -∗
+  instr (bv_unsigned SP_code_addr + 0x24) (Some Sally_Port.a24.a24) -∗
+  instr (bv_unsigned SP_code_addr + 0x28) (Some Sally_Port.a28.a28) -∗
+  instr (bv_unsigned SP_code_addr + 0x2c) (Some Sally_Port.a2c.a2c) -∗
+  instr (bv_unsigned P_code_addr) (Some P_entry.a0.a0) -∗
+  instr (bv_unsigned P_code_addr + 0x4) (Some P_entry.a4.a4) -∗
+  instr (bv_unsigned P_code_addr + 0x8) (Some P_entry.a8.a8) -∗
+  instr (bv_unsigned P_code_addr + 0xc) (Some P_entry.ac.ac) -∗
+  instr (bv_unsigned P_code_addr + 0x10) (Some P_entry.a10.a10) -∗
+  instr (bv_unsigned P_code_addr + 0x14) (Some P_entry.a14.a14) -∗
+  instr (bv_unsigned P_code_addr + 0x18) (Some P_entry.a18.a18) -∗
+  (∃ ins, instr ((bv_unsigned P_code_addr + 0x1c)) (Some ins)) -∗
+  instr_body (bv_unsigned SP_code_addr) (
+    Machine F_mtvec SP_pmpcfgs csr (<[3%nat := x10]> gpr) Pmem Fmem ∗
+    instr_pre (bv_unsigned ret_Encl_addr)
+      (∃ Pmem', Machine P_mtvec P_pmpcfgs csr0 (<[3%nat := x10]> gpr0) Pmem' Fmem)
+  ).
+Proof using F2E H csr0 csr0_length gpr0 gpr0_length ret_Encl_addr.
+  intros x10 csr gpr Pmem Fmem Hcsr Hgpr.
+  do 5 (destruct csr as [|? csr]; try inversion Hcsr).
+  do 6 (destruct gpr as [|? gpr]; try inversion Hgpr).
+  destruct csr0 as [|? csr0'] eqn:Hcsr0 ; try inversion csr0_length.
+  destruct gpr0 as [|? gpr0'] eqn:Hgpr0 ; try inversion gpr0_length.
+  do 4 (destruct csr0' as [|? csr0']; try inversion csr0_length).
+  do 5 (destruct gpr0' as [|? gpr0']; try inversion gpr0_length).
+  clear H1 H2 H3 H4 H5 H6 H7 H8 H9 H10 H11 H12 H13 H14 H15 H16 H17 H18 Hcsr Hgpr.
+  iStartProof.
+  iIntros "? ? ? ? ? ? ? ? ? ? ? ? ? ? ? ? ? ? ? Hret".
+  iPoseProof (SP2P_entry [b; b0; b1; b2] [b3; b4; b5; x10; b7] with "[$] [$] [$] [$] [$] [$] [$] [$] [$] [$] [$] [$]") as "HP2P_entry"; try done.
+  liARun.
+  iPoseProof (F2E x10 [ms; b0; b1; b2] [b3; b4; LET9; x10; b7] Pmem) as "HF2E".
+  liARun.
+  rewrite Hcsr0.
+  liARun.
+  iExists (mem', ())ₗ.
+  liARun.
+  rewrite Hgpr0.
+  liARun.
+  iFrame.
+  Unshelve. all: prepare_sidecond.
+  all: bv_solve.
+Qed.
+
+End SM.
+
+(* Information Flow: *)
+(* Ecall Enclave -> SM : Ecall Arguments by regs *)
+(* Ocall Enclave -> SM : Ecall Arguments by regs and host shared mem *)
+(* OS -> SM : Ecall Arguments by regs and host shared mem *)
+(* Firmware -> SM : well-defined subset of regs *)
+(* SM -> Firmware : Ecall Arguments / Exception No. / Int No. *)
+(* SM -> Enclave: *)
+(* Ecall / Non-Timer Trap : well-defined subset of regs *)
+(* Enclave Mgmt / Ocall Case: well-defined subset of regs and host shared *)
+(* mem *)
+
+
+(* Intgrity Guarantee: Enclave execution is fully decided by the Input *)
+(* and Enclave's Internal State. => the internal Enclave State are still *)
+(* same after the same Enclave instruction and Input and State even other *)
+(* things are different. *)
+(* => Input Seq and Init Config fully determines Enclave Execution. *)
+(* Input(OS via SM): subset of regs, host shared mem. *)
+(* Input(FM via SM): subset of regs. *)
+(* Input(Env via SM): subset of regs, host shared mem. *)
+
+(* Confidentiality: Firmware's execution is fully decided by the public *)
+(* State Vars. => the puibc State Vars are still same after the same *)
+(* Firmware instructions if they are same before, even the enclave state *)
+(* is different. *)
+(* => Public State Seq and Init fully determines the Firmware Execution. *)
+(* Output: the whole resulting machine State. The condition is that the *)
+(* observable part of State cannot leak. => same as before. *)
+(* observable part. *)
+
+(* Requirement: state after P_entry is fully determined by enclave's data *)
+(* region, the mem part except the general registers. *)
+(* Integrity: the firmware's state and input non-intefere the enclave's *)
+(* state. *)
+(* Confidentiality: the enclave's state and input non-interfere the *)
+(* resulting states observable by firmware. *)
+(* Inherit GPR and recover CSR. *)
