dorami/verification/model.v
@@ -1,0 +1,311 @@
+Require Export isla.riscv64.riscv64.
+From isla.dorami Require Export P2F.instrs.
+From isla.dorami Require Export exit_firmware.instrs.
+From isla.dorami Require Export Sally_Port.instrs.
+From isla.dorami Require Export P_entry.instrs.
+
+(* PMP grain and pmp addr mode *)
+(* | REGION       | ADDRESS    | LEN              | *)
+(* |--------------|------------|------------------| *)
+(* | DEVICE       | 0x00000000 | 0x80000000(2^31) | *)
+(* | P/CODE       | 0x80000000 | 0x20000(2^17)    | *)
+(* | F/CODE       | 0x80020000 | 0x1000(2^12)     | *)
+(* | SP/CODE      | 0x80021000 | 0x1000(2^12)     | *)
+(* | F/DATA       | 0x80022000 | 0x1000(2^12)     | *)
+(* | P/DATA       | 0x80040000 | 0x20000(2^17)    | *)
+(* | SP/CODE      | 0x80021000 | 0x1000(2^12)     | *)
+Definition device_addr := (BV 64 0x00000000).
+Definition P_code_addr := (BV 64 0x80000000).
+Definition F_code_addr := (BV 64 0x80020000).
+Definition F_code_end_addr := (BV 64 0x80020ffc).
+Definition SP_code_addr := (BV 64 0x80021000).
+Definition F_data_addr := (BV 64 0x80022000).
+Definition P_data_addr := (BV 64 0x80040000).
+
+Definition device_pmpaddr := (BV 64 0x7ffffff).
+Definition P_code_pmpaddr := (BV 64 0x80001fff).
+Definition F_code_pmpaddr := (BV 64 0x800200ff).
+Definition SP_code_pmpaddr := (BV 64 0x800210ff).
+Definition F_data_pmpaddr := (BV 64 0x800220ff).
+Definition P_data_pmpaddr := (BV 64 0x80041fff).
+
+(* PMP cfg when monitor, or osbi, or sally port executes. *)
+(* Region [0x0, DEVICE] is S/U-mode only. *)
+(* | REGION       | MONITOR EXEC | OSBI EXEC | SP EXEC  | *)
+(* |--------------|--------------|-----------|----------| *)
+(* | DEVICE       | 1e|AAWR      | 1e|AAWR   | 0        | *)
+(* | P/CODE       | 9D|LAAXR     | 98|LAA    | 0        | *)
+(* | F/CODE       | 98|LAA       | 9d|LAAXR  | 0        | *)
+(* | SP/CODE      | 98|LAA       | 98|LAA    | 0        | *)
+(* | F/DATA       | 98|LAA       | 9b|LAAWR  | 0        | *)
+(* | P/DATA       | 9b|LAAWR     | 98|LAA    | 0        | *)
+(* | SP/CODE      | 9d|LAAXR     | 9d|LAAXR  | 9d|LAAXR | *)
+
+(* PMP configuration in pmpcfg0 when P exec. *)
+Definition device_cfg_when_P := (BV 8 0x1e).
+Definition P_code_cfg_when_P := (BV 8 0x9d).
+Definition F_code_cfg_when_P := (BV 8 0x98).
+Definition SP_code_cfg_when_P := (BV 8 0x98).
+Definition F_data_cfg_when_P := (BV 8 0x98).
+Definition P_data_cfg_when_P := (BV 8 0x9b).
+
+(* PMP configuration in pmpcfg0 when firmware exec. *)
+Definition device_cfg_when_F := (BV 8 0x1e).
+Definition P_code_cfg_when_F := (BV 8 0x98).
+Definition F_code_cfg_when_F := (BV 8 0x9d).
+Definition SP_code_cfg_when_F := (BV 8 0x98).
+Definition F_data_cfg_when_F := (BV 8 0x9b).
+Definition P_data_cfg_when_F := (BV 8 0x98).
+
+(* PMP configuration in pmpcfg0 when sallyport exec. *)
+Definition components_cfg_when_SP := (BV 8 0x00).
+(* PMP configuration in pmpcfg0 when P_entry exec. *)
+Definition SP_code_cfg_when_P_entry := (BV 8 0x9d).
+(* PMP configuration of SallyPort in pmpcfg2 *)
+Definition SP_code_cfg := (BV 8 0x9d).
+
+Definition P_mtvec := P_code_addr.
+Definition P2F_code_size := 0x2c.
+Definition P_entry_code_size := 0x1c.
+Definition P2F_code_addr := bv_sub F_code_addr (BV 64 P2F_code_size).
+Definition F_mtvec := F_code_addr.
+
+(* pmp0cfg - pmp5cfg fields in pmpcfg0 register when P exec. *)
+Definition P_pmpcfgs :=
+  [device_cfg_when_P; P_code_cfg_when_P;
+   F_code_cfg_when_P; SP_code_cfg_when_P;
+   F_data_cfg_when_P; P_data_cfg_when_P].
+
+(* pmp0cfg - pmp5cfg fields in pmpcfg0 register when F exec. *)
+Definition F_pmpcfgs :=
+  [device_cfg_when_F; P_code_cfg_when_F;
+   F_code_cfg_when_F; SP_code_cfg_when_F;
+   F_data_cfg_when_F; P_data_cfg_when_F].
+
+(* pmp0cfg - pmp5cfg fields in pmpcfg0 register when SallyPort exec. *)
+Definition SP_pmpcfgs :=
+  [components_cfg_when_SP; components_cfg_when_SP;
+   components_cfg_when_SP; components_cfg_when_SP;
+   components_cfg_when_SP; components_cfg_when_SP].
+
+(* pmp0cfg - pmp5cfg fields in pmpcfg0 register when P_entry exec. *)
+Definition P_entry_pmpcfgs :=
+  [device_cfg_when_P; P_code_cfg_when_P;
+   F_code_cfg_when_P; SP_code_cfg_when_P_entry;
+   F_data_cfg_when_P; P_data_cfg_when_P].
+
+(* PMP registers that can be any value are existential values. *)
+(* We can add more existential pmpaddr and pmpcfg *)
+(* because the PMP entries with lower number have higher priority. *)
+Definition pmp_regs := [
+  (KindReg "pmpaddr0", ExactShape (RVal_Bits device_pmpaddr));
+  (KindReg "pmpaddr1", ExactShape (RVal_Bits P_code_pmpaddr));
+  (KindReg "pmpaddr2", ExactShape (RVal_Bits F_code_pmpaddr));
+  (KindReg "pmpaddr3", ExactShape (RVal_Bits SP_code_pmpaddr));
+  (KindReg "pmpaddr4", ExactShape (RVal_Bits F_data_pmpaddr));
+  (KindReg "pmpaddr5", ExactShape (RVal_Bits P_data_pmpaddr));
+  (KindReg "pmpaddr6", ExactShape (RVal_Bits (BV 64 0)));
+  (KindReg "pmpaddr7", ExactShape (RVal_Bits (BV 64 0)));
+  (KindReg "pmpaddr8", ExactShape (RVal_Bits SP_code_pmpaddr));
+  (KindReg "pmpaddr9", BitsShape 64);
+  (KindReg "pmpaddr10", BitsShape 64);
+  (KindReg "pmpaddr11", BitsShape 64);
+  (KindReg "pmpaddr12", BitsShape 64);
+  (KindReg "pmpaddr13", BitsShape 64);
+  (KindReg "pmpaddr14", BitsShape 64);
+  (KindReg "pmpaddr15", BitsShape 64);
+  (KindReg "pmp8cfg", StructShape ([("bits", ExactShape (RVal_Bits SP_code_cfg))]));
+  (KindReg "pmp9cfg", StructShape ([("bits", BitsShape 8)]));
+  (KindReg "pmp10cfg", StructShape ([("bits", BitsShape 8)]));
+  (KindReg "pmp11cfg", StructShape ([("bits", BitsShape 8)]));
+  (KindReg "pmp12cfg", StructShape ([("bits", BitsShape 8)]));
+  (KindReg "pmp13cfg", StructShape ([("bits", BitsShape 8)]));
+  (KindReg "pmp14cfg", StructShape ([("bits", BitsShape 8)]));
+  (KindReg "pmp15cfg", StructShape ([("bits", BitsShape 8)]))
+    ].
+
+(* All the configurations don't change *)
+Definition dorami_sys_regs := [
+  (KindReg "rv_enable_zfinx", ExactShape (RVal_Bool false));
+  (KindReg "rv_pmp_count", ExactShape (RegVal_I 16 64));
+  (KindReg "rv_pmp_grain", ExactShape (RegVal_I 10 64));
+  (KindReg "rv_enable_misaligned_access" , ExactShape (RVal_Bool false));
+  (KindReg "rv_ram_base" , ExactShape (RVal_Bits (BV 64 0x0000000080000000)));
+  (KindReg "rv_ram_size" , ExactShape (RVal_Bits (BV 64 0x0000000004000000)));
+  (KindReg "rv_rom_base" , ExactShape (RVal_Bits (BV 64 0x0000000000001000)));
+  (KindReg "rv_rom_size" , ExactShape (RVal_Bits (BV 64 0x0000000000000100)));
+  (KindReg "rv_clint_base" , ExactShape (RVal_Bits (BV 64 0x0000000002000000)));
+  (KindReg "rv_clint_size" , ExactShape (RVal_Bits (BV 64 0x00000000000c0000)));
+  (KindReg "rv_htif_tohost" , ExactShape (RVal_Bits (BV 64 0x0000000040001000)));
+  (KindReg "cur_privilege" , ExactShape (RVal_Enum "Machine"));
+  (* TODO: remove this *)
+  (KindReg "Machine" , ExactShape (RVal_Enum "Machine"));
+  (KindReg "mseccfg", ExactShape (RegVal_Struct [("bits", RVal_Bits (BV 64 0x07))]));
+  (KindReg "misa" , ExactShape (RegVal_Struct [("bits", RVal_Bits misa_bits)]))
+].
+
+(* All CSR *)
+Definition machine_csr (regs: list (bv 64)) :=
+  match regs with
+  | mstatus :: satp :: mcause :: mepc :: nil => [
+  (KindReg "mstatus", StructShape [("bits", ExactShape (RVal_Bits mstatus))]);
+  (KindReg "satp" , ExactShape (RVal_Bits satp));
+  (KindReg "mcause", StructShape [("bits", ExactShape (RVal_Bits mcause))]);
+  (KindReg "mepc", ExactShape (RVal_Bits mepc)) ]
+  | _ => nil end.
+
+(* All CSR with exitential values, used in the universal contract of F. *)
+(* TODO: remove it  *)
+Definition uni_csr := [
+  (KindReg "mstatus", StructShape [("bits", BitsShape 64)]);
+  (KindReg "satp" , BitsShape 64);
+  (KindReg "mcause", StructShape [("bits", BitsShape 64)]);
+  (KindReg "mepc", BitsShape 64)
+].
+
+(* All GPR *)
+Definition machine_gpr (regs: list (bv 64)) :=
+  match regs with
+  | x0::x1::x5::x10::x11::nil => [
+  (KindReg "x0", ExactShape (RVal_Bits x0));
+  (KindReg "x1", ExactShape (RVal_Bits x1));
+  (KindReg "x5", ExactShape (RVal_Bits x5));
+  (KindReg "x10", ExactShape (RVal_Bits x10));
+  (KindReg "x11", ExactShape (RVal_Bits x11)) ]
+  | _ => nil end.
+
+(* All CSR with exitential values, used in the universal contract of F. *)
+(* TODO: remove it  *)
+Definition uni_gpr := [
+  (KindReg "x0", BitsShape 64);
+  (KindReg "x1", BitsShape 64);
+  (KindReg "x5", BitsShape 64);
+  (KindReg "x10", BitsShape 64);
+  (KindReg "x11", BitsShape 64)
+].
+
+(* The two sets of definitions are equivalent. *)
+Lemma csr_equiv `{!islaG Σ} `{!threadG} :
+  reg_col uni_csr ⊣⊢ ∃ csr, ⌜length csr = 4%nat⌝ ∗ reg_col (machine_csr csr).
+Proof.
+  iSplit; rewrite /machine_csr /reg_col /=.
+  - liARun.
+    iExists (RegVal_Struct [("bits", RVal_Bits b)], b2, b1, b0, b, ())ₗ.
+    liARun.
+    iExists (RegVal_Struct [("bits", RVal_Bits b1)], ())ₗ.
+    by liARun.
+  - iIntros "[%csr [%Hcsr Hres]]".
+    do 5 (destruct csr as [|? csr]; try done); simpl.
+    iRevert "Hres".
+    liARun.
+    iExists (RegVal_Struct [("bits", RVal_Bits b)], ())ₗ.
+    iFrame.
+    by liARun.
+Qed.
+
+Lemma gpr_equiv `{!islaG Σ} `{!threadG} :
+  reg_col uni_gpr ⊣⊢ ∃ gpr, ⌜length gpr = 5%nat⌝ ∗ reg_col (machine_gpr gpr).
+Proof.
+  iSplit; rewrite /machine_gpr /reg_col /=.
+  - by liARun.
+  - iIntros "[%gpr [%Hgpr Hres]]".
+    do 6 (destruct gpr as [|? gpr]; try done); simpl.
+    iRevert "Hres".
+    liARun.
+    iExists (RVal_Bits b, ())ₗ.
+    iFrame.
+    by liARun.
+Qed.
+
+(* The Machine Model *)
+Definition Machine `{!islaG Σ} `{!threadG} (h: bv 64) (pmpcfgs: list (bv 8)) (csr gpr: list (bv 64)) (Pmem: bv (0x20000 * 8)) (Fmem: bv (0x1000 * 8)) : iProp Σ :=
+  match pmpcfgs with
+  | device_cfg :: monitor_code_cfg ::
+    osbi_code_cfg :: sp_code_cfg ::
+    osbi_data_cfg :: monitor_data_cfg :: nil =>
+  "mtvec" # "bits" ↦ᵣ RVal_Bits h ∗
+  "pmp0cfg" # "bits" ↦ᵣ RVal_Bits device_cfg ∗
+  "pmp1cfg" # "bits" ↦ᵣ RVal_Bits monitor_code_cfg  ∗
+  "pmp2cfg" # "bits" ↦ᵣ RVal_Bits osbi_code_cfg ∗
+  "pmp3cfg" # "bits" ↦ᵣ RVal_Bits sp_code_cfg ∗
+  "pmp4cfg" # "bits" ↦ᵣ RVal_Bits osbi_data_cfg ∗
+  "pmp5cfg" # "bits" ↦ᵣ RVal_Bits monitor_data_cfg ∗
+  "pmp6cfg" # "bits" ↦ᵣ RVal_Bits (BV 8 0) ∗
+  "pmp7cfg" # "bits" ↦ᵣ RVal_Bits (BV 8 0) ∗
+  reg_col dorami_sys_regs ∗ reg_col (machine_csr csr) ∗
+  reg_col (machine_gpr gpr) ∗ reg_col pmp_regs ∗
+  (bv_unsigned P_data_addr) ↦ₘ Pmem ∗
+  (bv_unsigned F_data_addr) ↦ₘ Fmem
+  | _ => emp end.
+
+Arguments Machine /.
+
+(* The P Compartment Model which doesn't have permission to *)
+(* F's data region compared with the Machine Model. *)
+Definition P `{!islaG Σ} `{!threadG}  (h: bv 64) (pmpcfgs: list (bv 8)) (csr gpr: list (bv 64)) (mem: bv (0x20000 * 8)): iProp Σ :=
+  match pmpcfgs, csr with
+  | device_cfg :: monitor_code_cfg ::
+    osbi_code_cfg :: sp_code_cfg ::
+    osbi_data_cfg :: monitor_data_cfg :: nil, mstatus :: other_csr =>
+  ⌜bv_extract 3 1 mstatus = (BV 1 0)⌝ ∗
+  "mtvec"# "bits" ↦ᵣ RVal_Bits h ∗
+  "pmp0cfg" # "bits" ↦ᵣ RVal_Bits device_cfg ∗
+  "pmp1cfg" # "bits" ↦ᵣ RVal_Bits monitor_code_cfg ∗
+  "pmp2cfg" # "bits" ↦ᵣ RVal_Bits osbi_code_cfg ∗
+  "pmp3cfg" # "bits" ↦ᵣ RVal_Bits sp_code_cfg ∗
+  "pmp4cfg" # "bits" ↦ᵣ RVal_Bits osbi_data_cfg ∗
+  "pmp5cfg" # "bits" ↦ᵣ RVal_Bits monitor_data_cfg ∗
+  "pmp6cfg" # "bits" ↦ᵣ RVal_Bits (BV 8 0) ∗
+  "pmp7cfg" # "bits" ↦ᵣ RVal_Bits (BV 8 0) ∗
+  reg_col dorami_sys_regs ∗ reg_col (machine_csr csr) ∗
+  reg_col (machine_gpr gpr) ∗ reg_col pmp_regs ∗
+  (bv_unsigned P_data_addr) ↦ₘ mem
+  | _, _ => emp end.
+
+Arguments P /.
+
+(* The F Compartment Model which doesn't have permission to *)
+(* P's data region compared with the Machine Model. *)
+Definition F `{!islaG Σ} `{!threadG}  (h: bv 64) (pmpcfgs: list (bv 8)) (csr gpr: list (bv 64)) (mem: bv (0x1000 * 8)): iProp Σ :=
+  match pmpcfgs with
+  | device_cfg :: monitor_code_cfg ::
+    osbi_code_cfg :: sp_code_cfg ::
+    osbi_data_cfg :: monitor_data_cfg :: nil =>
+  "mtvec"# "bits" ↦ᵣ RVal_Bits h ∗
+  "pmp0cfg" # "bits" ↦ᵣ RVal_Bits device_cfg ∗
+  "pmp1cfg" # "bits" ↦ᵣ RVal_Bits monitor_code_cfg ∗
+  "pmp2cfg" # "bits" ↦ᵣ RVal_Bits osbi_code_cfg ∗
+  "pmp3cfg" # "bits" ↦ᵣ RVal_Bits sp_code_cfg ∗
+  "pmp4cfg" # "bits" ↦ᵣ RVal_Bits osbi_data_cfg ∗
+  "pmp5cfg" # "bits" ↦ᵣ RVal_Bits monitor_data_cfg ∗
+  "pmp6cfg" # "bits" ↦ᵣ RVal_Bits (BV 8 0) ∗
+  "pmp7cfg" # "bits" ↦ᵣ RVal_Bits (BV 8 0) ∗
+  reg_col dorami_sys_regs ∗ reg_col (machine_csr csr) ∗
+  reg_col (machine_gpr gpr) ∗ reg_col pmp_regs ∗
+  (bv_unsigned F_data_addr) ↦ₘ mem
+  | _ => emp end.
+
+Arguments F /.
+
+(* The SallyPort Model which doesn't have permission to *)
+(* P's and F's data regions compared with the Machine Model. *)
+Definition SP `{!islaG Σ} `{!threadG} (h: bv 64) (pmpcfgs: list (bv 8)) (mie: bool) (csr gpr: list (bv 64)) : iProp Σ :=
+  match pmpcfgs, csr with
+  | device_cfg :: monitor_code_cfg ::
+    osbi_code_cfg :: sp_code_cfg ::
+    osbi_data_cfg :: monitor_data_cfg :: nil, mstatus::_ =>
+  ⌜if mie then True else bv_extract 3 1 mstatus = (BV 1 0)⌝ ∗
+  "mtvec"# "bits" ↦ᵣ RVal_Bits h ∗
+  "pmp0cfg" # "bits" ↦ᵣ RVal_Bits device_cfg ∗
+  "pmp1cfg" # "bits" ↦ᵣ RVal_Bits monitor_code_cfg ∗
+  "pmp2cfg" # "bits" ↦ᵣ RVal_Bits osbi_code_cfg ∗
+  "pmp3cfg" # "bits" ↦ᵣ RVal_Bits sp_code_cfg ∗
+  "pmp4cfg" # "bits" ↦ᵣ RVal_Bits osbi_data_cfg ∗
+  "pmp5cfg" # "bits" ↦ᵣ RVal_Bits monitor_data_cfg ∗
+  "pmp6cfg" # "bits" ↦ᵣ RVal_Bits (BV 8 0) ∗
+  "pmp7cfg" # "bits" ↦ᵣ RVal_Bits (BV 8 0) ∗
+  reg_col dorami_sys_regs ∗ reg_col (machine_csr csr) ∗
+  reg_col (machine_gpr gpr) ∗ reg_col pmp_regs
+  | _, _ => emp end.
+
+Arguments SP /.
