Makefile
@@ -19,24 +19,13 @@ update_etc:
 
 generate_dorami: update_etc
 	@echo "[islaris] dorami/P2F.dump"
-	@PATH=$$PWD/bin:$$PATH dune exec -- islaris dorami/P2F.dump -j 8 -o dorami/instructions/P2F --coqdir=isla.dorami.instructions.P2F --arch=riscv64
+	@PATH=$$PWD/bin:$$PATH dune exec -- islaris dorami/code/P2F.dump -j 8 -o dorami/instructions/P2F --coqdir=isla.dorami.instructions.P2F --arch=riscv64
 	@echo "[islaris] dorami/exit_firmware.dump"
-	@PATH=$$PWD/bin:$$PATH dune exec -- islaris dorami/exit_firmware.dump -j 8 -o dorami/instructions/exit_firmware --coqdir=isla.dorami.instructions.exit_firmware --arch=riscv64
+	@PATH=$$PWD/bin:$$PATH dune exec -- islaris dorami/code/exit_firmware.dump -j 8 -o dorami/instructions/exit_firmware --coqdir=isla.dorami.instructions.exit_firmware --arch=riscv64
 	@echo "[islaris] dorami/Sally_Port.dump"
-	@PATH=$$PWD/bin:$$PATH dune exec -- islaris dorami/Sally_Port.dump -j 8 -o dorami/instructions/Sally_Port --coqdir=isla.dorami.instructions.Sally_Port --arch=riscv64
+	@PATH=$$PWD/bin:$$PATH dune exec -- islaris dorami/code/Sally_Port.dump -j 8 -o dorami/instructions/Sally_Port --coqdir=isla.dorami.instructions.Sally_Port --arch=riscv64
 	@echo "[islaris] dorami/P_entry.dump"
-	@PATH=$$PWD/bin:$$PATH dune exec -- islaris dorami/P_entry.dump -j 8 -o dorami/instructions/P_entry --coqdir=isla.dorami.instructions.P_entry --arch=riscv64
-
-generate_test: update_etc
-#	@echo "[islaris] examples/test.dump"
-#	@PATH=$$PWD/bin:$$PATH dune exec -- islaris examples/test.dump -j 8 -o instructions/test --coqdir=isla.instructions.test --arch=riscv64
-	@echo "[islaris] examples/add.dump"
-	@PATH=$$PWD/bin:$$PATH dune exec -- islaris examples/add.dump -j 8 -o instructions/add --coqdir=isla.instructions.add --arch=riscv64
-.PHONY: generate_test
-
-my_test:
-	@dune build examples/add.vo --display short
-.PHONY: own_test
+	@PATH=$$PWD/bin:$$PATH dune exec -- islaris dorami/code/P_entry.dump -j 8 -o dorami/instructions/P_entry --coqdir=isla.dorami.instructions.P_entry --arch=riscv64
 
 generate_memory_instructions: examples/memory_instructions.dump update_etc
 	@echo "[islaris] $<"
